Prove the heap language is robustly safe.
I reverted to the ownp interface (cf. git:87abb52), dropped in
a new resource model, and proved robust safety.

theories/heap_lang/adequacy.v
@@ -1,26 +1,41 @@
-From iris.program_logic Require Export weakestpre adequacy gen_heap.
-From iris.heap_lang Require Export lifting.
 From iris.algebra Require Import auth.
-From iris.heap_lang Require Import proofmode notation.
+From iris.base_logic.lib Require Import auth.
+From iris.program_logic Require Export adequacy.
+From iris.heap_lang Require Export heap.
+From iris.heap_lang Require Import addenda robust_safety.
 From iris.proofmode Require Import tactics.
+Import addenda.ownp.
 
-Class heapPreG Σ := HeapPreG {
-  heap_preG_iris :> invPreG Σ;
-  heap_preG_heap :> gen_heapPreG loc val Σ
-}.
-
-Definition heapΣ : gFunctors := #[invΣ; gen_heapΣ loc val].
-Instance subG_heapPreG {Σ} : subG heapΣ Σ → heapPreG Σ.
-Proof. intros [? ?]%subG_inv; split; apply _. Qed.
-
-Definition heap_adequacy Σ `{heapPreG Σ} p e σ φ :
-  (∀ `{heapG Σ}, True ⊢ WP e @ p; ⊤ {{ v, ⌜φ v⌝ }}) →
-  adequate p e σ φ.
+Theorem heap_adequacy Σ `{heapPreG Σ} p e h φ :
+  (∀ `{heapG Σ}, heap_ctx ⊢ WP e @ p; ⊤ {{ v, ⌜φ v⌝ }}) →
+  adequate p e (good_state h) φ.
 Proof.
-  intros Hwp; eapply (wp_adequacy _ _); iIntros (?) "".
-  iMod (own_alloc (● to_gen_heap σ)) as (γ) "Hh".
-  { apply: auth_auth_valid. exact: to_gen_heap_valid. }
-  iModIntro. iExists (λ σ, own γ (● to_gen_heap σ)); iFrame.
-  set (Hheap := GenHeapG loc val Σ _ _ _ γ).
-  iApply (Hwp (HeapG _ _ _)).
+  intros Hwp. apply (ownP_adequacy _ _ _ _). iIntros (?) "Hσ".
+  iMod (heap_ctx_alloc with "Hσ") as (γ) "#Hh".
+  by iApply (Hwp (HeapG _ _ _ γ) with "Hh").
+Qed.
+
+Theorem heap_safety Σ `{heapPreG Σ} p e h1 t2 σ2 :
+  (∀ `{heapG Σ}, ∃ Φ, heap_ctx -∗ WP e @ p; ⊤ {{ Φ }}) →
+  rtc step ([e], good_state h1) (t2, σ2) → is_good σ2.
+Proof.
+  intros Hwp Hsteps.
+  apply: (ownP_invariance  _ p _ _ _ _ is_good) Hsteps=> /= ?.
+  iIntros "Hσ". iMod (heap_ctx_alloc with "Hσ") as (γ) "#Hh".
+  set G := (HeapG _  _ _ γ). iModIntro. iSplitL.
+  - case: (Hwp G) => Φ Hwp'. iExists Φ. by iApply Hwp'.
+  - by iApply (@heap_ctx_is_good _ G with "Hh").
+Qed.
+
+Corollary robust_safety Σ `{heapPreG Σ} C p e t2 σ2 :
+  adv_ctx C → is_closed [] e →
+  (∀ `{heapG Σ}, heap_ctx ⊢ WP e @ p; ⊤ {{ low }}) →
+  rtc step ([ctx_fill C e], good_state ∅) (t2, σ2) → is_good σ2.
+Proof.
+  move=>?? Hwp Hsteps. apply: (heap_safety Σ) Hsteps=>?.
+  exists low. iIntros "#Hh". rewrite (substitute_empty (ctx_fill _ _)).
+  iApply (robust_safety' with "[$Hh] [] [] []").
+  - by iApply adv_ctx_low.
+  - by rewrite low_env_empty.
+  - iAlways. iSplit. done. by iApply Hwp.
 Qed.
