theories/heap_lang/lifting.v
@@ -1,32 +1,11 @@
-From iris.program_logic Require Export weakestpre gen_heap.
+From iris.program_logic Require Export weakestpre ownp.
 From iris.program_logic Require Import ectx_lifting.
 From iris.heap_lang Require Export lang.
-From iris.heap_lang Require Import tactics.
+From iris.heap_lang Require Import tactics addenda.
 From iris.proofmode Require Import tactics.
 From iris.prelude Require Import fin_maps.
+Import addenda.ectx_language addenda.ectx_lifting addenda.ownp.
 Import uPred.
-
-(** Basic rules for language operations. *)
-
-Class heapG Σ := HeapG {
-  heapG_invG : invG Σ;
-  heapG_gen_heapG :> gen_heapG loc val Σ
-}.
-
-Instance heapG_irisG `{heapG Σ} : irisG heap_lang Σ := {
-  iris_invG := heapG_invG;
-  state_interp := gen_heap_ctx
-}.
-Global Opaque iris_invG.
-
-(** Override the notations so that scopes and coercions work out *)
-Notation "l ↦{ q } v" := (mapsto (L:=loc) (V:=val) l q v%V)
-  (at level 20, q at level 50, format "l  ↦{ q }  v") : uPred_scope.
-Notation "l ↦ v" :=
-  (mapsto (L:=loc) (V:=val) l 1 v%V) (at level 20) : uPred_scope.
-Notation "l ↦{ q } -" := (∃ v, l ↦{q} v)%I
-  (at level 20, q at level 50, format "l  ↦{ q }  -") : uPred_scope.
-Notation "l ↦ -" := (l ↦{1} -)%I (at level 20) : uPred_scope.
 
 (** The tactic [inv_head_step] performs inversion on hypotheses of the shape
 [head_step]. The tactic will discharge head-reductions starting from values, and
@@ -53,10 +32,13 @@ Local Hint Resolve alloc_fresh.
 Local Hint Resolve to_of_val.
 
 Section lifting.
-Context `{heapG Σ}.
+Context `{ownPG heap_lang Σ}.
 Implicit Types P Q : iProp Σ.
 Implicit Types Φ : val → iProp Σ.
+Implicit Types e : expr.
+Implicit Types v : val.
 Implicit Types efs : list expr.
+Implicit Types h : heap.
 Implicit Types σ : state.
 
 (** Bind. This bundles some arguments that wp_ectx_bind leaves as indices. *)
@@ -70,14 +52,52 @@ Lemma wp_bindi {p E e} Ki Φ :
 Proof. exact: weakestpre.wp_bind. Qed.
 
 (** Base axioms for core primitives of the language: Stateless reductions *)
-Lemma wp_fork p E e Φ :
-  ▷ Φ (LitV LitUnit) ∗ ▷ WP e @ p; ⊤ {{ _, True }} ⊢ WP Fork e @ p; E {{ Φ }}.
+Lemma wp_stuck_var x E Φ : True ⊢ WP Var x @ E ?{{ Φ }}.
 Proof.
-  rewrite -(wp_lift_pure_det_head_step (Fork e) (Lit LitUnit) [e]) //=; eauto.
-  - by rewrite later_sep -(wp_value _ _ _ (Lit _)) // big_sepL_singleton.
-  - intros; inv_head_step; eauto.
+  apply wp_lift_pure_head_stuck=>// -[|Ki ?] /= ????? ?.
+  by subst; inversion 1. by destruct Ki.
 Qed.
 
+Lemma wp_stuck_rec_open E f x e Φ :
+  ¬ is_closed (f :b: x :b: []) e → WP Rec f x e @ E ?{{ Φ }}%I.
+Proof.
+  move=>?.
+  apply wp_lift_pure_head_stuck; first by rewrite/=/to_val; case_decide.
+  move=>[|Ki ?] /= ????? ?. by subst; inversion 1. by destruct Ki.
+Qed.
+
+Definition is_rec e : Prop := ∃ f x erec, Rec f x erec = e.
+
+Global Instance is_rec_dec e : Decision (is_rec e).
+Proof.
+  rewrite /is_rec. case: e; try by intros; right; naive_solver.
+  move=>f x e. left. by exists f, x, e.
+Qed.
+
+Lemma wp_stuck_app_nrec E e1 v1 e2 v2 Φ :
+  to_val e1 = Some v1 → to_val e2 = Some v2 → ¬ is_rec e1 →
+  WP App e1 e2 @ E ?{{ Φ }}%I.
+Proof.
+  rewrite/is_rec=>???.
+  apply wp_lift_pure_head_stuck=>// -[|Ki ?] /= ????? Hfill Hstep.
+  { rewrite -Hfill in Hstep. inversion Hstep; subst. naive_solver. }
+  case: Ki Hfill=>//= ? [] ??; subst; apply: stuck_by_val Hstep; naive_solver.
+Qed.
+
+Lemma wp_stuck_app_open E e1 f x erec e2 v2 Φ :
+  e1 = Rec f x erec → to_val e2 = Some v2 → ¬ Closed (f :b: x :b: []) erec →
+  WP App e1 e2 @ E ?{{ Φ }}%I.
+Proof.
+  intros. apply wp_lift_pure_head_stuck=>//-[|Ki K] /= e ???? Hfill Hstep.
+  { rewrite -Hfill in Hstep. inversion Hstep. naive_solver. }
+  case: Ki Hfill=>//=.
+  - move=>e2' [] He1' He2'. subst.
+    have He: e = Rec f x erec by case: K He1' => //= -[].
+    rewrite He in Hstep. by inversion Hstep as [].
+  - move=>? [] ??; subst. apply: stuck_by_val Hstep. naive_solver.
+Qed.
+
+(* PDS: Misnamed. *)
 Lemma wp_rec p E f x erec e1 e2 Φ :
   e1 = Rec f x erec →
   is_Some (to_val e2) →
@@ -87,6 +107,15 @@ Proof.
   intros -> [v2 ?] ?. rewrite -(wp_lift_pure_det_head_step_no_fork (App _ _)
     (subst' x e2 (subst' f (Rec f x erec) erec))); eauto.
   intros; inv_head_step; eauto.
+Qed.
+
+Lemma wp_stuck_un_op op E e v Φ :
+  to_val e = Some v → un_op_eval op v = None →
+  WP UnOp op e @ E ?{{ Φ }}%I.
+Proof.
+  intros. apply wp_lift_pure_head_stuck=>//-[|Ki ?] /= ????? Hfill Hstep.
+  { rewrite -Hfill in Hstep. inversion Hstep; subst. naive_solver. }
+  case: Ki Hfill => //= ? [] ??; subst. apply: stuck_by_val Hstep. naive_solver.
 Qed.
 
 Lemma wp_un_op p E op e v v' Φ :
@@ -99,6 +128,16 @@ Proof.
   intros; inv_head_step; eauto.
 Qed.
 
+Lemma wp_stuck_bin_op E op e1 v1 e2 v2 Φ :
+  to_val e1 = Some v1 → to_val e2 = Some v2 →
+  bin_op_eval op v1 v2 = None →
+  WP BinOp op e1 e2 @ E ?{{ Φ }}%I.
+Proof.
+  intros. apply wp_lift_pure_head_stuck=>//-[|Ki ?] /= ????? Hfill Hstep.
+  { rewrite -Hfill in Hstep. inversion Hstep. naive_solver. }
+  case: Ki Hfill => //= ?? [] ???; subst; apply: stuck_by_val Hstep; naive_solver.
+Qed.
+
 Lemma wp_bin_op p E op e1 e2 v1 v2 v' Φ :
   to_val e1 = Some v1 → to_val e2 = Some v2 →
   bin_op_eval op v1 v2 = Some v' →
@@ -107,6 +146,23 @@ Proof.
   intros. rewrite -(wp_lift_pure_det_head_step_no_fork (BinOp op _ _) (of_val v'))
     -?wp_value'; eauto.
   intros; inv_head_step; eauto.
+Qed.
+
+Definition is_lit_bool e : Prop := ∃ b, Lit (LitBool b) = e.
+
+Global Instance is_lit_bool_dec e : Decision (is_lit_bool e).
+Proof.
+  rewrite /is_lit_bool. case: e; try by intros; right; naive_solver.
+  case; try by intros; right; naive_solver. move=>b. left. by exists b.
+Qed.
+
+Lemma wp_stuck_if E e v e1 e2 Φ :
+  to_val e = Some v → ¬ is_lit_bool e → WP If e e1 e2 @ E ?{{ Φ }}%I.
+Proof.
+  rewrite/is_lit_bool=>??.
+  apply wp_lift_pure_head_stuck=>//-[|Ki ?] /= ????? Hfill Hstep.
+  { rewrite -Hfill in Hstep. inversion Hstep; subst; naive_solver. }
+  case: Ki Hfill => //= ?? [] ???; subst. apply: stuck_by_val Hstep. naive_solver.
 Qed.
 
 Lemma wp_if_true p E e1 e2 Φ :
@@ -123,6 +179,25 @@ Proof.
   intros; inv_head_step; eauto.
 Qed.
 
+Definition is_pair_val e : Prop :=
+  ∃ e1 e2, is_Some (to_val e1) ∧ is_Some (to_val e2) ∧ e = Pair e1 e2.
+
+Global Instance is_pair_val_dec v : Decision (is_pair_val (of_val v)).
+Proof.
+  rewrite /is_pair_val. case: v; try by intros; right; naive_solver.
+  move=>v1 v2. left. do 2!eexists. by eauto using to_of_val.
+Qed.
+
+Lemma wp_stuck_fst E e v Φ :
+  to_val e = Some v → ¬ is_pair_val e → WP Fst e @ E ?{{ Φ }}%I.
+Proof.
+  rewrite/is_pair_val=>? Hp.
+  apply wp_lift_pure_head_stuck=>//-[|Ki ?] /= ?? e2 ?? Hfill Hstep.
+  { rewrite -Hfill in Hstep. inversion Hstep; subst.
+    apply: Hp. eexists e2, _. naive_solver. }
+  case: Ki Hfill => //= [] ?; subst. apply: stuck_by_val Hstep. naive_solver.
+Qed.
+
 Lemma wp_fst p E e1 v1 e2 Φ :
   to_val e1 = Some v1 → is_Some (to_val e2) →
   ▷ Φ v1 ⊢ WP Fst (Pair e1 e2) @ p; E {{ Φ }}.
@@ -132,6 +207,16 @@ Proof.
   intros; inv_head_step; eauto.
 Qed.
 
+Lemma wp_stuck_snd E e v Φ :
+  to_val e = Some v → ¬ is_pair_val e → WP Snd e @ E ?{{ Φ }}%I.
+Proof.
+  rewrite/is_pair_val=>? Hp.
+  apply wp_lift_pure_head_stuck=>//-[|Ki ?] /= ?? e2 ?? Hfill Hstep.
+  { rewrite -Hfill in Hstep. inversion Hstep; subst.
+    apply: Hp. exists e1, e2. naive_solver. }
+  case: Ki Hfill => //= [] ?; subst. apply: stuck_by_val Hstep. naive_solver.
+Qed.
+
 Lemma wp_snd p E e1 e2 v2 Φ :
   is_Some (to_val e1) → to_val e2 = Some v2 →
   ▷ Φ v2 ⊢ WP Snd (Pair e1 e2) @ p; E {{ Φ }}.
@@ -139,6 +224,25 @@ Proof.
   intros [v1 ?] ?.
   rewrite -(wp_lift_pure_det_head_step_no_fork (Snd _) e2) -?wp_value; eauto.
   intros; inv_head_step; eauto.
+Qed.
+
+Definition is_inj_val e : Prop :=
+  ∃ e', is_Some (to_val e') ∧ (e = InjL e' ∨ e = InjR e').
+
+Global Instance is_inj_val_dec v : Decision (is_inj_val (of_val v)).
+Proof.
+  rewrite /is_inj_val. destruct v; solve
+    [by right; naive_solver | by left; eexists; eauto using to_of_val].
+Qed.
+
+Lemma wp_stuck_case E e v e1 e2 Φ :
+  to_val e = Some v → ¬ is_inj_val e → WP Case e e1 e2 @ E ?{{ Φ }}%I.
+Proof.
+  rewrite/is_inj_val=>? Hs.
+  apply wp_lift_pure_head_stuck=>//-[|Ki ?] /= ????? Hfill Hstep.
+  { rewrite -Hfill in Hstep. inversion Hstep; subst;
+    apply: Hs; exists e0; naive_solver. }
+  case: Ki Hfill => //= ?? [] ???; subst. apply: stuck_by_val Hstep. naive_solver.
 Qed.
 
 Lemma wp_case_inl p E e0 e1 e2 Φ :
@@ -159,63 +263,108 @@ Proof.
   intros; inv_head_step; eauto.
 Qed.
 
-(** Heap *)
-Lemma wp_alloc p E e v :
-  to_val e = Some v →
-  {{{ True }}} Alloc e @ p; E {{{ l, RET LitV (LitLoc l); l ↦ v }}}.
+Lemma wp_assert p E e Φ :
+  WP e @ p; E {{ v, ⌜v = LitV (LitBool true)⌝ ∧ ▷ Φ (LitV LitUnit) }} -∗
+  WP Assert e @ p; E {{ Φ }}.
 Proof.
-  iIntros (<-%of_to_val Φ) "HΦ". iApply wp_lift_atomic_head_step_no_fork; auto.
-  iIntros (σ1) "Hσ !>"; iSplit; first by auto.
-  iNext; iIntros (v2 σ2 efs Hstep); inv_head_step.
-  iMod (@gen_heap_alloc with "Hσ") as "[Hσ Hl]"; first done.
-  iModIntro; iSplit=> //. iFrame. by iApply "HΦ".
+  change (Assert e) with (fill [AssertCtx] e). rewrite -wp_bind.
+  iIntros "He"; iApply (wp_wand with "[$He] []").
+  iIntros (v) "[% ?]". subst. simpl.
+  rewrite -(wp_lift_pure_det_head_step_no_fork (Assert _)) -?wp_value;
+    eauto.
+  intros; inv_head_step; eauto.
 Qed.
 
-Lemma wp_load p E l q v :
-  {{{ ▷ l ↦{q} v }}} Load (Lit (LitLoc l)) @ p; E {{{ RET v; l ↦{q} v }}}.
+Lemma wp_fork p E e Φ :
+  ▷ Φ (LitV LitUnit) ∗ ▷ WP e @ p; ⊤ {{ _, True }} ⊢ WP Fork e @ p; E {{ Φ }}.
 Proof.
-  iIntros (Φ) ">Hl HΦ". iApply wp_lift_atomic_head_step_no_fork; auto.
-  iIntros (σ1) "Hσ !>". iDestruct (@gen_heap_valid with "Hσ Hl") as %?.
-  iSplit; first by eauto.
-  iNext; iIntros (v2 σ2 efs Hstep); inv_head_step.
-  iModIntro; iSplit=> //. iFrame. by iApply "HΦ".
+  rewrite -(wp_lift_pure_det_head_step (Fork e) (Lit LitUnit) [e]) //=; eauto.
+  - by rewrite later_sep -(wp_value _ _ _ (Lit _)) // big_sepL_singleton.
+  - intros; inv_head_step; eauto.
 Qed.
 
-Lemma wp_store p E l v' e v :
-  to_val e = Some v →
-  {{{ ▷ l ↦ v' }}} Store (Lit (LitLoc l)) e @ p; E {{{ RET LitV LitUnit; l ↦ v }}}.
+(** Base axioms for stateful reduction. *)
+Lemma wp_alloc_pst p E σ h v :
+  heap_of σ = h →
+  {{{ ▷ ownP σ }}} Alloc (of_val v) @ p; E
+  {{{ l, RET LitV (LitLoc l); ⌜h !! l = None⌝ ∧ ownP (hupd σ (<[l:=v]>h)) }}}.
 Proof.
-  iIntros (<-%of_to_val Φ) ">Hl HΦ".
-  iApply wp_lift_atomic_head_step_no_fork; auto.
-  iIntros (σ1) "Hσ !>". iDestruct (@gen_heap_valid with "Hσ Hl") as %?.
-  iSplit; first by eauto. iNext; iIntros (v2 σ2 efs Hstep); inv_head_step.
-  iMod (@gen_heap_update with "Hσ Hl") as "[$ Hl]".
-  iModIntro. iSplit=>//. by iApply "HΦ".
+  iIntros (? Φ) "HP HΦ".
+  iApply (ownP_lift_atomic_head_step (Alloc (of_val v)) σ); eauto.
+  iFrame "HP". iNext. iIntros (e2 σ2 ef) "% HP". inv_head_step.
+  iSplitL; last by iApply big_sepL_nil. iApply "HΦ". by iSplit.
 Qed.
 
-Lemma wp_cas_fail p E l q v' e1 v1 e2 v2 :
-  to_val e1 = Some v1 → to_val e2 = Some v2 → v' ≠ v1 →
-  {{{ ▷ l ↦{q} v' }}} CAS (Lit (LitLoc l)) e1 e2 @ p; E
-  {{{ RET LitV (LitBool false); l ↦{q} v' }}}.
+Definition is_loc e : Prop := ∃ l, e = Lit (LitLoc l).
+
+Global Instance is_loc_dec e : Decision (is_loc e).
 Proof.
-  iIntros (<-%of_to_val <-%of_to_val ? Φ) ">Hl HΦ".
-  iApply wp_lift_atomic_head_step_no_fork; auto.
-  iIntros (σ1) "Hσ !>". iDestruct (@gen_heap_valid with "Hσ Hl") as %?.
-  iSplit; first by eauto. iNext; iIntros (v2' σ2 efs Hstep); inv_head_step.
-  iModIntro; iSplit=> //. iFrame. by iApply "HΦ".
+  rewrite /is_loc. case: e; try by intros; right; naive_solver.
+  case; try by intros; right; naive_solver. move=>l. left. by exists l.
 Qed.
 
-Lemma wp_cas_suc p E l e1 v1 e2 v2 :
-  to_val e1 = Some v1 → to_val e2 = Some v2 →
-  {{{ ▷ l ↦ v1 }}} CAS (Lit (LitLoc l)) e1 e2 @ p; E
-  {{{ RET LitV (LitBool true); l ↦ v2 }}}.
+Lemma wp_stuck_load E e v Φ :
+  to_val e = Some v → ¬ is_loc e → WP Load e @ E ?{{ Φ }}%I.
 Proof.
-  iIntros (<-%of_to_val <-%of_to_val Φ) ">Hl HΦ".
-  iApply wp_lift_atomic_head_step_no_fork; auto.
-  iIntros (σ1) "Hσ !>". iDestruct (@gen_heap_valid with "Hσ Hl") as %?.
-  iSplit; first by eauto. iNext; iIntros (v2' σ2 efs Hstep); inv_head_step.
-  iMod (@gen_heap_update with "Hσ Hl") as "[$ Hl]".
-  iModIntro. iSplit=>//. by iApply "HΦ".
+  rewrite/is_loc=>??.
+  apply wp_lift_pure_head_stuck=>//-[|Ki ?] /= ????? Hfill Hstep.
+  { rewrite -Hfill in Hstep. inversion Hstep; subst. naive_solver. }
+  case: Ki Hfill=> //= [] ?; subst. apply: stuck_by_val Hstep. naive_solver.
+Qed.
+
+Lemma wp_load_pst p E σ h l v :
+  heap_of σ = h → h !! l = Some v →
+  {{{ ▷ ownP σ }}} Load (Lit (LitLoc l)) @ p; E {{{ RET v; ownP σ }}}.
+Proof.
+  intros ?? Φ. apply ownP_lift_atomic_det_head_step_no_fork; eauto.
+  intros; inv_head_step; eauto.
+Qed.
+
+Lemma wp_stuck_store E e1 v1 e2 v2 Φ :
+  to_val e1 = Some v1 → to_val e2 = Some v2 → ¬ is_loc e1 →
+  WP Store e1 e2 @ E ?{{ Φ }}%I.
+Proof.
+  rewrite/is_loc=>???.
+  apply wp_lift_pure_head_stuck=>//-[|Ki ?] /= ????? Hfill Hstep.
+  { rewrite -Hfill in Hstep. inversion Hstep; subst. naive_solver. }
+  case: Ki Hfill=> //= ? [] ??; subst; apply: stuck_by_val Hstep; naive_solver.
+Qed.
+
+Lemma wp_store_pst p E σ h l v v' :
+  heap_of σ = h → h !! l = Some v' →
+  {{{ ▷ ownP σ }}} Store (Lit (LitLoc l)) (of_val v) @ p; E
+  {{{ RET LitV LitUnit; ownP (hupd σ (<[l:=v]>h)) }}}.
+Proof.
+  intros. apply ownP_lift_atomic_det_head_step_no_fork; eauto.
+  intros; inv_head_step; eauto.
+Qed.
+
+Lemma wp_stuck_cas E e0 v0 e1 v1 e2 v2 Φ :
+  to_val e0 = Some v0 → to_val e1 = Some v1 → to_val e2 = Some v2 →
+  ¬ is_loc e0 → WP CAS e0 e1 e2 @ E ?{{ Φ }}%I.
+Proof.
+  rewrite/is_loc=>????.
+  apply wp_lift_pure_head_stuck=>//-[|Ki ?] /= ????? Hfill Hstep.
+  { rewrite -Hfill in Hstep. inversion Hstep; subst; naive_solver. }
+  case: Ki Hfill=> //= ?? [] ???; subst; apply: stuck_by_val Hstep; naive_solver.
+Qed.
+
+Lemma wp_cas_fail_pst p E σ h l v1 v2 v' :
+  heap_of σ = h → h !! l = Some v' → v' ≠ v1 →
+  {{{ ▷ ownP σ }}} CAS (Lit (LitLoc l)) (of_val v1) (of_val v2) @ p; E
+  {{{ RET LitV $ LitBool false; ownP σ }}}.
+Proof.
+  intros. apply ownP_lift_atomic_det_head_step_no_fork; eauto.
+  intros; inv_head_step; eauto.
+Qed.
+
+Lemma wp_cas_suc_pst p E σ h l v1 v2 :
+  heap_of σ = h → h !! l = Some v1 →
+  {{{ ▷ ownP σ }}} CAS (Lit (LitLoc l)) (of_val v1) (of_val v2) @ p; E
+  {{{ RET LitV $ LitBool true; ownP (hupd σ (<[l:=v2]>h)) }}}.
+Proof.
+  intros. apply ownP_lift_atomic_det_head_step_no_fork; eauto.
+  intros; inv_head_step; eauto.
 Qed.
 
 (** Proof rules for derived constructs *)
