theories/heap_lang/addenda.v
@@ -1,0 +1,348 @@
+From iris.proofmode Require Import tactics.
+
+Module fin_maps.	(* cf. ../prelude/fin_maps.v *)
+From iris.prelude Require Import fin_maps.
+Section union.
+  Context `{FinMap K M}.
+
+  Lemma lookup_union_Some_r' {A} (m1 m2 : M A) i x :
+    m1 !! i = None → m2 !! i = Some x → (m1 ∪ m2) !! i = Some x.
+  Proof. rewrite lookup_union_Some_raw; intuition. Qed.
+
+  (* PDS: There's likely a much shorter proof. *)
+  Lemma delete_insert_union {A} (m1 m2 : M A) i x :
+    m1 !! i = Some x → m2 !! i = None → m1 ∪ m2 = delete i m1 ∪ <[i:=x]> m2.
+  Proof.
+    transitivity (m1 ∪ {[i:=x]} ∪ m2).
+    { f_equal. apply map_eq => i'.
+      case: (decide (i = i'))=> [<-|?]; first by simplify_map_eq.
+      case EQ: (m1 !! i')=> [hv|]; first by simplify_map_eq.
+      symmetry. apply lookup_union_None. by simplify_map_eq. }
+    rewrite (insert_union_singleton_l m2 i x) assoc. f_equal.
+    apply map_eq => i'. case: (decide (i = i'))=> [<-|?]; simplify_map_eq.
+    { symmetry. rewrite lookup_union_Some_raw. right. by simplify_map_eq. }
+    case EQ: (m1 !! i')=>[hv|]; simplify_map_eq.
+    { symmetry. rewrite lookup_union_Some_raw. left. by simplify_map_eq. }
+    by transitivity (None : option A); [| symmetry];
+      apply lookup_union_None; simplify_map_eq.
+  Qed.
+End union.
+
+Section difference.
+  Context `{FinMap K M}.
+
+  Lemma map_difference_empty {A} (m : M A) : m ∖ ∅ = m.
+  Proof.
+    apply/map_eq=>i. case EQ: (_ !! _)=>[x|].
+    - by move: EQ =>/lookup_difference_Some [] ->.
+    - move: EQ=>/lookup_difference_None [->//|].
+      by rewrite lookup_empty=>/is_Some_None.
+  Qed.
+End difference.
+End fin_maps.
+
+Module list.	(* cf. ../prelude/list.v *)
+Section list.
+  Context `{EqDecision A}.
+  Context (P : A → Prop) `{∀ x, Decision (P x)}.
+
+  Lemma filter_cons l x :
+    filter P (x :: l) = if decide (P x) then x :: filter P l else filter P l.
+  Proof. by []. Qed.
+
+  Lemma foldr_cons {B} (f : A → B → B) (b : B) (a : A) (l : list A) :
+    foldr f b (a :: l) = f a (foldr f b l).
+  Proof. by []. Qed.
+
+  Lemma foldr_filter {B} (R : relation B) `{!Equivalence R}
+      (f : A → B → B) (b : B) (l : list A) `{!Proper ((=) ==> R ==> R) f}
+      (Hf : ∀ a b, ¬ P a → R b (f a b)) :
+    R (foldr f b (filter P l)) (foldr f b l).
+  Proof.
+    elim: l=> // a l IH. rewrite filter_cons. case: (decide _)=> /= ?.
+    - f_equiv. exact: IH.
+    - etrans. exact: IH. exact: Hf.
+  Qed.
+End list.
+End list.
+
+Module gmap.	(* cf. ../algebra/gmap.v *)
+Section gmap.
+  From iris.algebra Require Import gmap.
+
+  Context `{Countable K} {A : cmraT}.
+  Implicit Types m : gmap K A.
+
+  Lemma insert_op_r i x m1 m2 :
+    m1 !! i = None → <[i:=x]>(m1  ⋅ m2) = m1 ⋅ (<[i:=x]>m2).
+  Proof.
+    intros Hdom. rewrite (insert_merge_r _ _ _ _ _ x).
+    done. by rewrite Hdom.
+  Qed.
+  Lemma insert_op_l i x m1 m2 :
+    m2 !! i = None → <[i:=x]>(m1  ⋅ m2) = (<[i:=x]>m1) ⋅ m2.
+  Proof.
+    intros Hdom. rewrite (insert_merge_l _ _ _ _ _ x).
+    done. by rewrite Hdom.
+  Qed.
+End gmap.
+End gmap.
+
+Module csum.	(* cf. ../algebra/csum.v *)
+Section csum.
+  From iris.algebra Require Import csum.
+
+  Context {A B : cmraT}.
+  Implicit Types a : A.
+  Implicit Types b : B.
+
+  Lemma Cinl_included a1 a2 :
+    @included (csum A B) _ _ (Cinl a1) (Cinl a2) ↔ a1 ≼ a2.
+  Proof.
+    rewrite csum_included; split; last by move=>?; right; left; do 2!eexists.
+    case => //; case => //; last by move=> [? [? [? _]]]; exfalso.
+    by move=> [? [? [[->] [[->] ?]]]].
+  Qed.
+
+  Lemma Cinr_included b1 b2 :
+    @included (csum A B) _ _ (Cinr b1) (Cinr b2) ↔ b1 ≼ b2.
+  Proof.
+    rewrite csum_included; split; last by move=>?; right; right; do 2!eexists.
+    case => //; case => //; first by move=> [? [? [? _]]]; exfalso.
+    by move=> [? [? [[->] [[->] ?]]]].
+  Qed.
+
+  Lemma csum_equivE (x y : csum A B) :
+    x ≡ y ↔ (match x, y with
+              | Cinl a, Cinl a' => a ≡ a'
+              | Cinr b, Cinr b' => b ≡ b'
+              | CsumBot, CsumBot => True
+              | _, _ => False
+              end).
+  Proof.
+    split; first by destruct 1.
+    by destruct x, y; try destruct 1; try constructor.
+  Qed.
+End csum.
+End csum.
+
+Module option.	(* cf. ../base_logic/primitive.v:/option_equivI *)
+Section option.
+  From iris.algebra Require Import ofe.
+  Context {A : ofeT}.
+
+  Lemma option_equivE (mx my : option A) :
+    mx ≡ my ↔ match mx, my with
+               | Some x, Some y => x ≡ y | None, None => True | _, _ => False
+               end.
+  Proof. split. by destruct 1. by destruct mx, my; try constructor. Qed.
+End option.
+End option.
+
+
+Module auth.	(* cf. ../base_logic/lib/auth.v *)
+Section auth.
+  From iris.base_logic.lib Require Import auth.
+  Context `{invG Σ, authG Σ A}.
+  Context {T : Type} `{!Inhabited T}.
+  Context (f : T → A) (φ : T → iProp Σ).
+  Implicit Types N : namespace.
+  Implicit Types P Q R : iProp Σ.
+  Implicit Types a b : A.
+  Implicit Types t u : T.
+  Implicit Types γ : gname.
+
+  Lemma auth_acc_strong E γ a :
+    ▷ auth_inv γ f φ ∗ auth_own γ a ={E}=∗ ∃ t,
+      ⌜✓ (f t)⌝ ∗ ⌜a ≼ f t⌝ ∗ ▷ φ t ∗ ∀ u b,
+      ⌜(f t, a) ~l~> (f u, b)⌝ ∗ ▷ φ u ={E}=∗ ▷ auth_inv γ f φ ∗ auth_own γ b.
+  Proof.
+    iIntros "[Hinv Hγf]". rewrite /auth_inv /auth_own.
+    iDestruct "Hinv" as (t) "[>Hγa Hφ]".
+    iModIntro. iExists t.
+    iDestruct (own_valid_2 with "Hγa Hγf") as % [? ?]%auth_valid_discrete_2.
+    iSplit; first done. iSplit; first done. iFrame. iIntros (u b) "[% Hφ]".
+    iMod (own_update_2 with "Hγa Hγf") as "[Hγa Hγf]".
+    { eapply auth_update; eassumption. }
+    iModIntro. iFrame. iExists u. iFrame.
+  Qed.
+
+  Lemma auth_acc E γ a :
+    ▷ auth_inv γ f φ ∗ auth_own γ a ={E}=∗ ∃ t,
+      ⌜a ≼ f t⌝ ∗ ▷ φ t ∗ ∀ u b,
+      ⌜(f t, a) ~l~> (f u, b)⌝ ∗ ▷ φ u ={E}=∗ ▷ auth_inv γ f φ ∗ auth_own γ b.
+  Proof.
+    rewrite auth_acc_strong. iIntros ">H !>". iDestruct "H" as (t) "(_&?&?)".
+    iExists t. by iFrame.
+  Qed.
+
+  Lemma auth_open_strong E N γ a :
+    ↑N ⊆ E →
+    auth_ctx γ N f φ ∗ auth_own γ a ={E,E∖↑N}=∗ ∃ t,
+      ⌜✓ (f t)⌝ ∗ ⌜a ≼ f t⌝ ∗ ▷ φ t ∗ ∀ u b,
+      ⌜(f t, a) ~l~> (f u, b)⌝ ∗ ▷ φ u ={E∖↑N,E}=∗ auth_own γ b.
+  Proof.
+    iIntros (?) "[#? Hγf]". rewrite /auth_ctx. iInv N as "Hinv" "Hclose".
+    (* The following is essentially a very trivial composition of the accessors
+       [auth_acc] and [inv_open] -- but since we don't have any good support
+       for that currently, this gets more tedious than it should, with us having
+       to unpack and repack various proofs.
+       TODO: Make this mostly automatic, by supporting "opening accessors
+       around accessors". *)
+    iMod (auth_acc_strong with "[$Hinv $Hγf]") as (t) "(?&?&?&HclAuth)".
+    iModIntro. iExists t. iFrame. iIntros (u b) "H".
+    iMod ("HclAuth" $! u b with "H") as "(Hinv & ?)".
+    by iMod ("Hclose" with "Hinv").
+  Qed.
+
+  Lemma auth_open E N γ a :
+    ↑N ⊆ E →
+    auth_ctx γ N f φ ∗ auth_own γ a ={E,E∖↑N}=∗ ∃ t,
+      ⌜a ≼ f t⌝ ∗ ▷ φ t ∗ ∀ u b,
+      ⌜(f t, a) ~l~> (f u, b)⌝ ∗ ▷ φ u ={E∖↑N,E}=∗ auth_own γ b.
+  Proof.
+    move=>?; rewrite auth_open_strong //. iIntros ">H !>".
+    iDestruct "H" as (t) "(_&?&?&?)". iExists t. by iFrame.
+  Qed.
+End auth.
+Arguments auth_open_strong {_ _ _} [_] {_} [_] _ _ _ _ _ _ _.
+Arguments auth_open {_ _ _} [_] {_} [_] _ _ _ _ _ _ _.
+End auth.
+
+Module ectx_language.	(* cf. ../program_logic/ectx_language.v *)
+From iris.program_logic Require Import ectx_language.
+Section ectx_language.
+  Context {expr val ectx state} {Λ : EctxLanguage expr val ectx state}.
+  Implicit Types (e : expr) (K : ectx).
+
+  Lemma stuck_by_val K e σ e' σ' efs :
+    is_Some (to_val (fill K e)) → ¬ head_step e σ e' σ' efs.
+  Proof.
+    intros Hv Hnv%val_stuck%(fill_not_val K). apply: is_Some_None.
+    by rewrite Hnv in Hv.
+  Qed.
+End ectx_language.
+End ectx_language.
+
+Module ectx_lifting.	(* cf. ../program_logic/ectx_lifting.v *)
+From iris.program_logic Require Import lifting ectx_lifting.
+Section ectx_lifting.
+
+  Context {expr val ectx state} {Λ : EctxLanguage expr val ectx state}.
+  Context `{irisG (ectx_lang expr) Σ}.
+  Implicit Types p : pbit.
+  Implicit Types P : iProp Σ.
+  Implicit Types Φ : val → iProp Σ.
+  Implicit Types v : val.
+  Implicit Types e : expr.
+
+  Definition head_progress (e : expr) (σ : state) :=
+    is_Some(to_val e) ∨ ∃ K e', e = fill K e' ∧ head_reducible e' σ.
+
+  Lemma progress_head_progress e σ :
+    language.progress e σ → head_progress e σ.
+  Proof.
+    case=>[?|Hred]; first by left.
+    right. move: Hred=> [] e' [] σ' [] efs [] K e1' e2' EQ EQ' Hstep. subst.
+    exists K, e1'. split; first done. by exists e2', σ', efs.
+  Qed.
+  Hint Resolve progress_head_progress.
+
+  Lemma wp_lift_head_stuck E Φ e :
+    to_val e = None →
+    (∀ σ, state_interp σ ={E,∅}=∗ ⌜¬ head_progress e σ⌝)
+    ⊢ WP e @ E ?{{ Φ }}.
+  Proof.
+    iIntros (?) "H". iApply wp_lift_stuck; first done.
+    iIntros (σ) "Hσ". iMod ("H" $! _ with "Hσ") as "%". iModIntro. by auto.
+  Qed.
+
+  Lemma wp_lift_pure_head_stuck `{Inhabited state} E Φ e :
+    to_val e = None →
+    (∀ K e1 σ1 e2 σ2 efs, e = fill K e1 → ¬ head_step e1 σ1 e2 σ2 efs) →
+    WP e @ E ?{{ Φ }}%I.
+  Proof.
+    iIntros (Hnv Hnstep). iApply wp_lift_head_stuck; first done.
+    iIntros (σ) "_". iMod (fupd_intro_mask' E ∅) as "_"; first set_solver.
+    iModIntro. iPureIntro. case; first by rewrite Hnv; case.
+    move=>[] K [] e1 [] Hfill [] e2 [] σ2 [] efs /= Hstep. exact: Hnstep.
+  Qed.
+
+  (* Derived identically to wp_lift_pure_stuck. PDS: Dead. *)
+  Lemma wp_lift_pure_head_stuck_old `{Inhabited state} E Φ e :
+    (∀ σ, ¬ head_progress e σ) →
+    True ⊢ WP e @ E ?{{ Φ }}.
+  Proof.
+    iIntros (Hstuck). iApply wp_lift_head_stuck.
+    - destruct(to_val e) as [v|] eqn:He; last done.
+      by exfalso; apply (Hstuck inhabitant); left; exists v.
+    - iIntros (σ) "_". iMod (fupd_intro_mask' E ∅) as "_"; first set_solver.
+      iModIntro. iPureIntro. apply Hstuck.
+  Qed.
+End ectx_lifting.
+End ectx_lifting.
+
+Module adequacy.
+From iris.base_logic Require Import big_op soundness.
+From iris.program_logic Require Import adequacy.
+
+Theorem wp_invariance Σ Λ `{invPreG Σ} p e σ1 t2 σ2 φ :
+  (∀ `{Hinv : invG Σ},
+     True ={⊤}=∗ ∃ stateI : state Λ → iProp Σ,
+       let _ : irisG Λ Σ := IrisG _ _ Hinv stateI in
+       stateI σ1 ∗ (∃ Φ, WP e @ p; ⊤ {{ Φ }}) ∗ (stateI σ2 ={⊤,∅}=∗ ⌜φ⌝)) →
+  rtc step ([e], σ1) (t2, σ2) →
+  φ.
+Proof.
+  intros Hwp [n ?]%rtc_nsteps.
+  eapply (soundness (M:=iResUR Σ) _ (S (S (S n)))); iIntros "".
+  rewrite Nat_iter_S. iMod wsat_alloc as (Hinv) "[Hw HE]".
+  rewrite {1}fupd_eq in Hwp; iMod (Hwp with "[$Hw $HE]") as ">(Hw & HE & Hwp)".
+  iDestruct "Hwp" as (Istate) "(HIstate & Hwp & Hclose)".
+  iDestruct "Hwp" as (Φ) "Hwp".
+  iModIntro. iNext. iApply (@wptp_invariance _ _ (IrisG _ _ Hinv Istate)); eauto.
+  iFrame "Hw HE Hwp HIstate Hclose". by iApply big_sepL_nil.
+Qed.
+End adequacy.
+
+Module ownp.
+From iris.algebra Require Import auth.
+From iris.program_logic Require Import ownp.
+Import adequacy.
+
+Theorem ownP_invariance Σ `{ownPPreG Λ Σ} p e σ1 t2 σ2 φ :
+  (∀ `{ownPG Λ Σ},
+    ownP σ1 ={⊤}=∗ (∃ Φ, WP e @ p; ⊤ {{ Φ }}) ∗ |={⊤,∅}=> ∃ σ', ownP σ' ∧ ⌜φ σ'⌝) →
+  rtc step ([e], σ1) (t2, σ2) →
+  φ σ2.
+Proof.
+  intros Hwp Hsteps. eapply (wp_invariance Σ Λ p e σ1 t2 σ2 _)=> //.
+  iIntros (?) "". iMod (own_alloc (● (Excl' (σ1 : leibnizC _)) ⋅ ◯ (Excl' σ1)))
+    as (γσ) "[Hσ Hσf]"; first done.
+  iExists (λ σ, own γσ (● (Excl' (σ:leibnizC _)))). iFrame "Hσ".
+  iMod (Hwp (OwnPG _ _ _ _ γσ) with "[Hσf]") as "[$ H]"; first by rewrite /ownP.
+  iIntros "!> Hσ". iMod "H" as (σ2') "[Hσf %]". rewrite/ownP.
+  iDestruct (own_valid_2 with "Hσ Hσf")
+    as %[->%Excl_included%leibniz_equiv _]%auth_valid_discrete_2; auto.
+Qed.
+
+Section _ectx_lifting.
+  From iris.program_logic Require Import lifting ectx_lifting.
+  Import ectx_lifting.
+  Hint Resolve progress_head_progress.
+
+  Context {expr val ectx state} {Λ : EctxLanguage expr val ectx state}.
+  Context `{ownPG (ectx_lang expr) Σ}.
+  Implicit Types p : pbit.
+  Implicit Types Φ : val → iProp Σ.
+  Implicit Types e : expr.
+
+  Lemma ownP_lift_head_stuck E Φ e :	(* PDS: Dead. *)
+    (|={E,∅}=> ∃ σ, ⌜¬ head_progress e σ⌝ ∗ ▷ ownP σ)
+    ⊢ WP e @ E ?{{ Φ }}.
+  Proof.
+    iIntros "H". iApply ownP_lift_stuck. iMod "H" as (σ) "[% Hσ]".
+    iModIntro. iExists σ. iFrame. by eauto.
+  Qed.
+End _ectx_lifting.
+End ownp.
