theories/heap_lang/heap.v
@@ -1,0 +1,704 @@
+From iris.prelude Require Import gmultiset.
+From iris.algebra Require Import auth gmap csum agree.
+From iris.algebra Require Export gset frac.
+From iris.base_logic.lib Require Export invariants.
+From iris.base_logic.lib Require Import own auth fractional.
+From iris.base_logic Require Import big_op.
+From iris.heap_lang Require Export lifting.
+From iris.heap_lang Require addenda.
+From iris.proofmode Require Import tactics.
+Import uPred.
+Import addenda.fin_maps.
+Import addenda.option addenda.gmap addenda.csum.
+Import addenda.auth.
+
+Local Hint Resolve to_of_val.
+
+(** The CMRA we need. *)
+Local Notation heap := (gmap loc val).
+Definition heapN : namespace := nroot .@ "heap".
+Definition heapUR : ucmraT :=
+  gmapUR loc (csumR (prodR fracR (agreeR valC)) unitR).
+Local Notation Hval q v := (Cinl (q%Qp, to_agree v)).
+Local Notation Lval := (Cinr ()).
+
+Class heapG Σ := HeapG {
+  heap_ownP_inG :> ownPG heap_lang Σ;
+  heap_inG :> authG Σ heapUR;
+  heap_name : gname
+}.
+
+Class heapPreG Σ := HeapPreG {
+  heap_preG_ownP_inG : ownPPreG heap_lang Σ;
+  heap_preG_inG : authG Σ heapUR
+}.
+(*
+ * Lower priority than heapG's instances so the occurrence of
+ * [heap_ctx] in the statement of [heap_adequacy] refers to the
+ * "inner" [heapG] rather than the "outer" [heapPreG].
+ *)
+Existing Instance heap_preG_ownP_inG | 30.
+Existing Instance heap_preG_inG | 30.
+
+Definition heapΣ : gFunctors := #[ownPΣ state; authΣ heapUR].
+Instance subG_heapPreG {Σ} : subG heapΣ Σ → heapPreG Σ.
+Proof. intros [??]%subG_inv; constructor; apply _. Qed.
+
+(** * Heap resources and invariant *)
+Section definitions.
+  Context `{ownPG heap_lang Σ, authG Σ heapUR} (γ : gname).
+  Implicit Types l : loc.
+  Implicit Types q : Qp.
+  Implicit Types v : val.
+  Implicit Types h : heap.
+
+  (** High locations. *)
+  Definition mapsto_def l q v : iProp Σ := auth_own γ {[l := Hval q v]}.
+  Definition mapsto_aux : { x | x = @mapsto_def }. by eexists. Qed.
+  Definition mapsto := proj1_sig mapsto_aux.
+  Definition mapsto_eq : @mapsto = @mapsto_def := proj2_sig mapsto_aux.
+
+  (** Low locations. *)
+  Definition lowloc_def l : iProp Σ := auth_own γ {[l := Lval]}.
+  Definition lowloc_aux : { x | x = @lowloc_def }. by eexists. Qed.
+  Definition lowloc := proj1_sig lowloc_aux.
+  Definition lowloc_eq : @lowloc = @lowloc_def := proj2_sig lowloc_aux.
+
+  (**
+    Low values. When proving a function low, one may use any
+    invariant.
+  *)
+  Definition lowval_pre (rec : val -c> iProp Σ) : val -c> iProp Σ := λ v,
+    match v with
+    | RecV f x e _ => □ ▷ ∀ v, rec v -∗
+      WP subst' x (of_val v) (subst' f (Rec f x e) e) ?{{ rec }}
+    | LitV (LitLoc l) => lowloc l
+    | LitV (LitInt _ | LitBool _ | LitUnit) => True
+    | PairV v1 v2 => ▷(rec v1 ∗ rec v2)
+    | InjLV v | InjRV v => ▷(rec v)
+    end%I.
+
+  Instance lowval_pre_contractive : Contractive lowval_pre.
+  Proof.
+    rewrite /lowval_pre=> n rec rec' Hrec ?.
+    repeat (f_contractive || f_equiv); apply Hrec.
+  Qed.
+
+  Definition lowval_def : val → iProp Σ := fixpoint lowval_pre.
+  Definition lowval_aux : { x | x = @lowval_def }. by eexists. Qed.
+  Definition lowval := proj1_sig lowval_aux.
+  Definition lowval_eq : @lowval = @lowval_def := proj2_sig lowval_aux.
+
+  Lemma lowval_unfold v : lowval v ≡ lowval_pre lowval v.
+  Proof. rewrite lowval_eq. apply (fixpoint_unfold lowval_pre). Qed.
+
+  (**
+    Invariant: The state is good and maps every high location to its
+    value and every low location to a low value.
+  *)
+  Definition to_high : heap → heapUR := fmap (λ v, Hval 1 v).
+  Definition to_low : heap → heapUR  := fmap (λ _, Lval).
+  Definition to_heap (a : heap * heap) : heapUR :=
+    let: (h, h') := a in to_high h ⋅ to_low h'.
+  Definition hinv' (a : heap * heap) : iProp Σ :=
+    let: (h, h') := a in
+    (ownP (good_state (h ∪ h')) ∗ [∗ map] v ∈ h', lowval v)%I.
+
+  Lemma hinv_alloc h : ownP (good_state h) -∗ ▷ hinv' (h, ∅).
+  Proof.
+    rewrite /hinv' right_id big_sepM_empty right_id. exact: later_intro.
+  Qed.
+
+  Lemma to_heap_valid h : ✓ to_heap (h, ∅).
+  Proof. move=>l. rewrite lookup_op !lookup_fmap. by case (h !! l). Qed.
+
+  Definition heap_ctx' : iProp Σ := auth_ctx γ heapN to_heap hinv'.
+  Global Instance heap_ctx_persistent : PersistentP heap_ctx'.
+  Proof. apply _. Qed.
+End definitions.
+Typeclasses Opaque mapsto lowloc lowval.
+Instance: Params (@mapsto) 2.
+Instance: Params (@lowloc) 2.
+Instance: Params (@lowval) 3.
+Instance: Params (@heap_ctx') 3.
+
+Notation "l ↦{ q } v" := (mapsto heap_name l q v)
+  (at level 20, q at level 50, format "l  ↦{ q }  v") : uPred_scope.
+Notation "l ↦ v" := (mapsto heap_name l 1 v) (at level 20) : uPred_scope.
+
+Notation "l ↦{ q } -" := (∃ v, l ↦{q} v)%I
+  (at level 20, q at level 50, format "l  ↦{ q }  -") : uPred_scope.
+Notation "l ↦ -" := (l ↦{1} -)%I (at level 20) : uPred_scope.
+
+Notation heap_ctx := (heap_ctx' heap_name).
+Local Notation hinv := (hinv' heap_name).
+
+(** Allocating the invariant. *)
+(** We cannot use [auth_alloc] as [hinv] depends on the ghost name. *)
+Lemma heap_ctx_alloc `{ownPG heap_lang Σ, authG Σ heapUR} E h :
+  ownP (good_state h) ={E}=∗ ∃ γ, heap_ctx' γ.
+Proof.
+  iIntros "Hσ". set h' := to_heap (h, ∅).
+  iMod (own_alloc (Auth (Excl' h') h')) as (γ) "Ha".
+  { split. done. exact: to_heap_valid. }
+  set hinv_γ := @hinv' _ _ _ γ.
+  iRevert "Ha"; rewrite auth_both_op; iIntros "[Ha _]".
+  iDestruct (@hinv_alloc _ _ _ γ with "Hσ") as "Hσ".
+  iMod (inv_alloc heapN _ (auth_inv γ to_heap hinv_γ) with "[Ha Hσ]") as "#?".
+  { iNext. rewrite/auth_inv. iExists (h, ∅). by iFrame. }
+  iModIntro. iExists γ. by rewrite/heap_ctx'/auth_ctx.
+Qed.
+
+(** Observing good states. *)
+Lemma heap_ctx_is_good `{heapG Σ} E :
+ ↑heapN ⊆ E → heap_ctx ={E,∅}=∗ ∃ σ, ownP σ ∧ ⌜is_good σ⌝.
+Proof.
+  iIntros (?) "Hinv". iMod (fupd_intro_mask' _ (↑heapN)) as "_"; first done.
+  iMod (auth_empty heap_name) as "Ha".
+  iMod (auth_open with "[$Hinv $Ha]") as ([h h']) "(_&[>Hh _]&_)";
+    first done.
+  iExists _; iFrame. by rewrite subseteq_empty_difference_L.
+Qed.
+
+(** * Low integrity predicates *)
+Class LowIntegrity Σ (A : Type) := Low {
+  low : A → iProp Σ;
+  low_persistent a :> PersistentP (low a)
+}.
+Arguments Low {_ _} _ _.
+Arguments low {_ _ _} _ : simpl never.
+Instance: Params (@low) 3.
+
+Section low.
+  Context `{heapG Σ}.
+
+  (** Low locations are defined by [lowloc]. *)
+  Global Instance lowloc_persistent l : PersistentP (lowloc heap_name l).
+  Proof. rewrite lowloc_eq /lowloc_def. apply _. Qed.
+  Global Instance loc_low : LowIntegrity Σ loc := Low (lowloc heap_name) _.
+  Global Instance loc_low_timeless (l : loc) : TimelessP (low l).
+  Proof. rewrite /low/= lowloc_eq /lowloc_def. apply _. Qed.
+
+  Lemma low_loc l : low l ⊣⊢ lowloc heap_name l.
+  Proof. by []. Qed.
+
+  (** Literals other than locations are automatically low. *)
+  Definition lowlit : base_lit → iProp Σ :=
+    λ lit, match lit with
+    | LitInt _ | LitBool _ | LitUnit => True
+    | LitLoc l => low l
+    end%I.
+  Global Instance lowlit_persistent lit : PersistentP (lowlit lit).
+  Proof. case: lit; apply _. Qed.
+  Global Instance lit_low : LowIntegrity Σ base_lit := Low lowlit _.
+  Global Instance lit_low_timeless (lit : base_lit) : TimelessP (low lit).
+  Proof. case: lit; apply _. Qed.
+
+  Lemma low_lit lit :
+    low lit ⊣⊢
+    match lit with
+    | LitInt _ | LitBool _ | LitUnit => True
+    | LitLoc l => low l
+    end.
+  Proof. by []. Qed.
+
+  (**
+    A (syntactically) low expression contains neither assertions nor
+    high locations. (We reserve assertions for verified code.)
+  *)
+  Definition lowexpr : expr → iProp Σ :=
+    fix rec e := match e with
+    | Var _ => True
+    | Assert _ => False
+    | Lit lit => low lit
+    | Rec _ _ e | UnOp _ e | Fst e | Snd e | InjL e | InjR e
+    | Fork e | Alloc e | Load e
+      => rec e
+    | App e1 e2 | BinOp _ e1 e2 | Pair e1 e2 | Store e1 e2 => rec e1 ∗ rec e2
+    | If e1 e2 e3 | Case e1 e2 e3 | CAS e1 e2 e3
+      => rec e1 ∗ rec e2 ∗ rec e3
+    end%I.
+  Global Instance lowexpr_persistent e : PersistentP (lowexpr e).
+  Proof.
+    rewrite/lowexpr; elim: e=>//; rewrite-/lowexpr; by apply _.
+  Qed.
+  Global Instance lowexpr_low : LowIntegrity Σ expr := Low lowexpr _.
+  Global Instance lowexpr_low_timeless (e : expr) : TimelessP (low e).
+  Proof.
+    rewrite/lowexpr; elim: e=>//; rewrite-/lowexpr; by apply _.
+  Qed.
+
+  Lemma low_expr e :
+    low e ⊣⊢
+    match e with
+    | Var _ => True
+    | Assert _ => False
+    | Lit lit => low lit
+    | Rec _ _ e | UnOp _ e | Fst e | Snd e | InjL e | InjR e
+    | Fork e | Alloc e | Load e
+      => low e
+    | App e1 e2 | BinOp _ e1 e2 | Pair e1 e2 | Store e1 e2 => low e1 ∗ low e2
+    | If e1 e2 e3 | Case e1 e2 e3 | CAS e1 e2 e3
+      => low e1 ∗ low e2 ∗ low e3
+    end.
+  Proof. by case: e. Qed.
+
+  (** Low values are defined by [lowval]. *)
+  Global Instance lowval_persistent v : PersistentP (lowval heap_name v).
+  Proof.
+    iIntros "Hv". iLöb as "IH" forall (v). rewrite lowval_unfold /lowval_pre.
+    destruct v.
+    - by iDestruct "Hv" as "#Hv".
+    - by iDestruct "Hv" as "#Hv".
+    - rewrite always_later. iNext. iDestruct "Hv" as "(Hv1&Hv2)".
+      iDestruct ("IH" with "* Hv1") as "#Hv1'".
+      iDestruct ("IH" with "* Hv2") as "#Hv2'". iClear "Hv1 Hv2".
+      iAlways. by iFrame "#".
+    - rewrite always_later. iNext. by iSpecialize ("IH" with "* Hv").
+    - rewrite always_later. iNext. by iSpecialize ("IH" with "* Hv").
+  Qed.
+  Global Instance val_low : LowIntegrity Σ val := Low (lowval heap_name) _.
+
+  Lemma lowval_low v : low v ⊣⊢ lowval heap_name v.
+  Proof. by []. Qed.
+
+  Lemma low_val v :
+    low v ⊣⊢
+    match v with
+    | RecV f x e _ => □ ▷ ∀ v, low v -∗
+      WP subst' x (of_val v) (subst' f (Rec f x e) e) ?{{ low }}
+    | LitV lit => low lit
+    | PairV v1 v2 => ▷ (low v1 ∗ low v2)
+    | InjLV v | InjRV v => ▷ low v
+    end.
+  Proof. by destruct v; rewrite lowval_low lowval_unfold. Qed.
+
+  Lemma low_recv_alt f x e `{!Closed (f :b: x :b: []) e} :
+    low (RecV f x e) ⊣⊢
+    □ ▷ ∀ e2 v2 Φ, ⌜to_val e2 = Some v2⌝ -∗ low v2 -∗
+      (∀ v, low v -∗ Φ v) -∗ WP subst' x e2 (subst' f (Rec f x e) e) ?{{ Φ }}.
+  Proof.
+    rewrite low_val. iSplit.
+    - iIntros "#Hv !#". iNext. iIntros (e2 v2 Φ) "% #Hv2 HΦ".
+      iApply (wp_wand with "[Hv Hv2] [$HΦ]"). rewrite -(of_to_val e2 v2) //.
+      by iApply ("Hv" with "[$Hv2]").
+    - iIntros "#Hv !#". iNext. iIntros (v2) "#Hv2".
+      iApply ("Hv" with "[%] [$Hv2] []"). done. by iIntros.
+  Qed.
+
+  Global Instance val_low_lit_timeless lit : TimelessP (low (LitV lit)).
+  Proof. by rewrite /TimelessP low_val lit_low_timeless. Qed.
+(* Also sound, but who cares?
+  Global Instance low_rec_except_0 f x e `{!Closed (f :b: x :b: []) e} :
+    IsExcept0 (low (RecV f x e)).
+  Global Instance low_pair_except_0 v1 v2 : IsExcept0 (low (PairV v1 v2)).
+  Global Instance low_inj_l_except_0 v : IsExcept0 (low (InjLV v)).
+  Global Instance low_inj_r_except_0 v : IsExcept0 (low (InjRV v)).
+*)
+End low.
+
+(** * Bookkeeping lemmas *)
+Section bookkeeping.
+  Context `{heapG Σ}.
+  Implicit Types l : loc.
+  Implicit Types q : Qp.
+  Implicit Types v : val.
+  Implicit Types h : heap.
+
+  Remark to_heap_disjoint h h' : ✓ to_heap (h, h') → h ⊥ₘ h'.
+  Proof.
+    move=>Hv. rewrite map_disjoint_spec=>l ? ? EQ EQ'; move/(_ l): Hv.
+    by rewrite /to_heap lookup_op /to_high /to_low 2!lookup_fmap EQ EQ'.
+  Qed.
+
+  Lemma lookup_to_high_None h l : h !! l = None → to_high h !! l = None.
+  Proof. by rewrite /to_high lookup_fmap=> ->. Qed.
+  Lemma lookup_to_low_None h l : h !! l = None → to_low h !! l = None.
+  Proof. by rewrite /to_low lookup_fmap=> ->. Qed.
+  Lemma lookup_to_heap_None h h' l :
+    (h ∪ h') !! l = None → to_heap (h, h') !! l = None.
+  Proof.
+    move=> /lookup_union_None [??].
+    by rewrite lookup_op lookup_to_high_None ?lookup_to_low_None.
+  Qed.
+
+  Lemma lookup_to_high_Some h l v :
+    h !! l = Some v → to_high h !! l = Some(Hval 1 v).
+  Proof. by rewrite /to_high lookup_fmap=>->. Qed.
+  Lemma lookup_to_low_Some h l v : h !! l = Some v → to_low h !! l = Some Lval.
+  Proof. by rewrite /to_low lookup_fmap=>->. Qed.
+  Lemma lookup_to_heap_Some h h' l v :
+    h !! l = Some v → h' !! l = None → to_heap (h, h') !! l = Some (Hval 1 v).
+  Proof.
+    rewrite /to_heap lookup_op.
+    by move=>/lookup_to_high_Some->/lookup_to_low_None->.
+  Qed.
+
+  Lemma to_heap_high_included h h' l q v :
+    ✓ to_heap (h, h') → {[l := Hval q v]} ≼ to_heap (h, h') →
+    h !! l = Some v ∧ h' !! l = None.
+  Proof.
+    rewrite singleton_included => /(_ l) Hv [] u []; move: Hv.
+    rewrite !lookup_op /to_high /to_low !lookup_fmap.
+    case EQ: (h !! l)=>[vh|]; case EQ': (h' !! l)=>[vl|] /=.
+    - by rewrite -Some_op Some_valid.
+    - rewrite right_id.
+      intros Hv (?&Heq&Heq')%(equiv_Some_inv_r _ _ u) Hinc; last done.
+      apply (inj Some) in Heq. move: Heq Heq' Hinc => <- => Heq.
+      case/Some_included.
+      + by move: Heq=><- /csum_equivE [] _ /= /to_agree_inj
+          /leibniz_equiv_iff ->.
+      + move=> Hinc; move: Hinc Heq.
+        case/csum_included; first by move=>->/csum_equivE.
+        case; last by move=> [?] [?] [].
+        move=> [[qa ua]] [[qb ub]] [] [<-<-] [] ->.
+        move=> /prod_included/= [] _ Hinc.
+        move=>/csum_equivE/= [] /= _ => Heq.
+        rewrite <- Heq in Hinc.
+        by move: Hinc => /to_agree_included /leibniz_equiv_iff ->.
+    - rewrite left_id => _ Heq. apply (inj Some) in Heq. rewrite <- Heq.
+      case/Some_included; first by move=>/csum_equivE.
+      case/csum_included; first done.
+      case. by move=> [?] [?] [] _ []. by move=> [?] [?] [].
+    - rewrite right_id. by move=> _ /option_equivE.
+  Qed.
+
+  Lemma to_heap_low_included h h' l :
+    ✓ to_heap (h, h') → {[l := Lval]} ≼ to_heap (h, h') →
+    h !! l = None ∧ is_Some(h' !! l).
+  Proof.
+    rewrite singleton_included => /(_ l) Hv [] u []; move: Hv.
+    rewrite !lookup_op /to_high /to_low !lookup_fmap.
+    case EQ: (h !! l)=>[vh|]; case EQ': (h' !! l)=>[vl|] /=.
+    - by rewrite -Some_op Some_valid.
+    - rewrite right_id => _ Heq Hinc. apply Some_equiv_inj in Heq.
+      case/Some_included: Hinc Heq; first by move=><- /csum_equivE.
+      case/csum_included; first by move=>-> /csum_equivE.
+      case; first by move=> [?] [?] [].
+      by move=> [?] [?] [] _ [] -> _ /csum_equivE.
+    - move=>_ _ _. split. done. by exists vl.
+    - rewrite right_id. by move=> _ /option_equivE.
+  Qed.
+
+  Lemma to_heap_high_insert h h' l v :
+    h' !! l = None →
+    to_heap (<[l:=v]> h, h') = <[l:=Hval 1 v]>(to_heap (h, h')).
+  Proof.
+    move=>?. rewrite /to_heap /to_high fmap_insert. apply/map_eq => l'.
+    case: (decide (l = l'))=> [<-|?].
+    - rewrite insert_op_l //. by rewrite lookup_to_low_None.
+    - by rewrite lookup_op lookup_insert_ne // lookup_insert_ne // -lookup_op.
+  Qed.
+
+  Lemma to_heap_low_insert h h' l v :
+    h !! l = None → to_heap (h, <[l:=v]> h') = <[l:=Lval]>(to_heap (h, h')).
+  Proof.
+    move=>?. rewrite /to_heap /to_low fmap_insert. apply/map_eq=> l'.
+    case: (decide (l = l'))=> [<-|?].
+    - rewrite insert_op_r //. by rewrite lookup_to_high_None.
+    - by rewrite lookup_op lookup_insert_ne // lookup_insert_ne // -lookup_op.
+  Qed.
+
+  Lemma to_heap_low_insert_override h h' l v1 v2 :
+    h' !! l = Some v1 → to_heap (h, h') = to_heap (h, <[l:=v2]> h').
+  Proof.
+    move=>Hlow. apply/map_eq=> l'. rewrite 2!lookup_op. f_equiv.
+    rewrite /to_low 2!lookup_fmap. case: (decide (l = l')) =>[<-|?].
+    - by rewrite Hlow lookup_insert.
+    - by rewrite lookup_insert_ne.
+  Qed.
+
+  Lemma to_heap_delete h h' l :
+    h' !! l = None →
+    delete l (to_heap (h, h')) = to_heap (delete l h, h').
+  Proof.
+    move=>Hdom. rewrite /to_heap /to_high fmap_delete.
+    apply/map_eq=> l'. rewrite lookup_op. case: (decide (l = l'))=> [<-|?].
+    - by rewrite !lookup_delete lookup_to_low_None.
+    - by rewrite lookup_delete_ne // lookup_delete_ne // -lookup_op.
+  Qed.
+
+  Lemma to_heap_mark_low h h' l v :
+    ✓ to_heap (h, h') → {[l := Hval 1 v]} ≼ to_heap (h, h') →
+    (to_heap (h, h'), {[l := Hval 1 v]}) ~l~>
+    (to_heap (delete l h, <[l:=v]> h'), {[l := Lval]}).
+  Proof.
+    move=>Hv /to_heap_high_included -/(_ Hv)[_ ?].
+    etransitivity; first by apply delete_singleton_local_update, _.
+    rewrite to_heap_delete // to_heap_low_insert; last by rewrite lookup_delete.
+    apply alloc_singleton_local_update; last done.
+    apply lookup_to_heap_None, lookup_union_None. by rewrite lookup_delete.
+  Qed.
+
+  Lemma to_heap_alloc_high h h' l v :
+    (h ∪ h') !! l = None →
+    (to_heap (h, h'), ∅) ~l~> (to_heap (<[l:=v]> h, h'), {[l := Hval 1 v]}).
+  Proof.
+    move=>Hdom.
+    rewrite to_heap_high_insert; last by move: Hdom=>/lookup_union_None[].
+    apply alloc_singleton_local_update; last done.
+    by apply lookup_to_heap_None.
+  Qed.
+
+  Lemma to_heap_store_high h h' l v1 v2 :
+    ✓ to_heap (h, h') → h !! l = Some v1 → h' !! l = None →
+    (to_heap (h, h'), {[l := Hval 1 v1]}) ~l~>
+    (to_heap (<[l:=v2]> h, h'), {[l := Hval 1 v2]}).
+  Proof.
+    move=>???. rewrite to_heap_high_insert //.
+    eapply singleton_local_update; first exact: lookup_to_heap_Some.
+    exact: exclusive_local_update.
+  Qed.
+
+  Lemma hinv_intro h h' :
+    ownP (good_state (h ∪ h')) -∗ ([∗ map] v ∈ h', low v) -∗ hinv (h, h').
+  Proof. rewrite/hinv. by iIntros; iFrame. Qed.
+
+  Lemma hinv_high h h' l v :
+    ownP (good_state (<[l:=v]> (h ∪ h'))) -∗ ([∗ map] v ∈ h', low v) -∗
+    hinv (<[l:=v]> h, h').
+  Proof. rewrite/hinv insert_union_l. by iIntros; iFrame. Qed.
+
+  Lemma hinv_mark_low h h' l v :
+    ✓ to_heap (h, h') → {[l := Hval 1 v]} ≼ to_heap (h, h') →
+    ▷ ownP (good_state (h ∪ h')) -∗
+    ▷ low v -∗ ▷ ([∗ map] v' ∈ h', low v') -∗ ▷ hinv (delete l h, <[l:=v]>h').
+  Proof.
+    move=>Hv /to_heap_high_included -/(_ Hv)[??]. rewrite/hinv.
+    iIntros "Hh Hv Hlow". rewrite -delete_insert_union //.
+    iFrame. rewrite 2!big_sepM_later big_sepM_insert //. by iFrame.
+  Qed.
+
+  Lemma hinv_store_low h h' l v1 v2 :
+    h !! l = None → h' !! l = Some v1 →
+    ownP (good_state (<[l:=v2]> (h ∪ h'))) -∗
+    ([∗ map] v ∈ h', low v) -∗ low v2 -∗ hinv (h, <[l:=v2]> h').
+  Proof.
+    move=>??.
+    rewrite /hinv insert_union_r // big_sepM_insert_override_2 //.
+    iIntros "? Hlow ?". iFrame. iApply "Hlow". eauto.
+  Qed.
+End bookkeeping.
+
+(** * Heap interface *)
+Section heap.
+  Context `{heapG Σ}.
+  Implicit Types l : loc.
+  Implicit Types q : Qp.
+  Implicit Types v : val.
+  Implicit Types h : heap.
+
+  (** High and low locations are disjoint. *)
+  Lemma high_not_low l q v : l ↦{q} v ∗ low l ⊢ False.
+  Proof.
+    by rewrite mapsto_eq low_loc lowloc_eq
+      -auth_own_op auth_own_valid discrete_valid
+      op_singleton singleton_valid.
+  Qed.
+
+  (** High locations enjoy their usual properties. *)
+  Global Instance mapsto_timeless l q v : TimelessP (l ↦{q} v).
+  Proof. rewrite mapsto_eq. apply _. Qed.
+  Global Instance mapsto_fractional l v : Fractional (λ q, l ↦{q} v)%I.
+  Proof.
+    intros p q. by rewrite mapsto_eq -auth_own_op
+      op_singleton Cinl_op pair_op agree_idemp.
+  Qed.
+  Global Instance mapsto_as_fractional l q v :
+    AsFractional (l ↦{q} v) (λ q, l ↦{q} v)%I q.
+  Proof. split. done. apply _. Qed.
+
+  Lemma mapsto_agree l q1 q2 v1 v2 : l ↦{q1} v1 ∗ l ↦{q2} v2 ⊢ ⌜v1 = v2⌝.
+  Proof.
+    rewrite mapsto_eq -auth_own_op auth_own_valid discrete_valid
+      op_singleton singleton_valid Cinl_op pair_op.
+    by f_equiv=> -[] _ /agree_op_inv/to_agree_inj/leibniz_equiv_iff.
+  Qed.
+
+  Global Instance heap_ex_mapsto_fractional l : Fractional (λ q, l ↦{q} -)%I.
+  Proof.
+    intros p q. iSplit.
+    - iDestruct 1 as (v) "[H1 H2]". iSplitL "H1"; eauto.
+    - iIntros "[H1 H2]". iDestruct "H1" as (v1) "H1". iDestruct "H2" as (v2) "H2".
+      iDestruct (mapsto_agree with "[$H1 $H2]") as %->. iExists v2. by iFrame.
+  Qed.
+  Global Instance heap_ex_mapsto_as_fractional l q :
+    AsFractional (l ↦{q} -) (λ q, l ↦{q} -)%I q.
+  Proof. split. done. apply _. Qed.
+
+  Lemma mapsto_valid l q v : l ↦{q} v ⊢ ✓ q.
+  Proof.
+    rewrite mapsto_eq /mapsto_def auth_own_valid !discrete_valid
+      singleton_valid.
+    by apply pure_mono=> -[].
+  Qed.
+  Lemma mapsto_valid_2 l q1 q2 v1 v2 : l ↦{q1} v1 ∗ l ↦{q2} v2 ⊢ ✓ (q1 + q2)%Qp.
+  Proof.
+    iIntros "[H1 H2]". iDestruct (mapsto_agree with "[$H1 $H2]") as %->.
+    iApply (mapsto_valid l _ v2). by iFrame.
+  Qed.
+
+  (** High locations containing low values may be marked low. *)
+  Lemma heap_mark_low E l v :
+    ↑heapN ⊆ E →
+    heap_ctx -∗ ▷ l ↦ v -∗ ▷ low v ={E}=∗ low l.
+  Proof.
+    iIntros (?) "#Hinv >Hl Hv". rewrite /heap_ctx mapsto_eq /mapsto_def.
+    iMod (auth_open_strong with "[$Hinv $Hl]")
+      as ([h h']) "(%&%&[Hh Hlow]&Hcl)"; first done.
+    iDestruct (hinv_mark_low with "Hh Hv Hlow") as "Hh"; [done|done|].
+    iMod ("Hcl" with "* [Hh]") as "Ha".
+    - iFrame. iPureIntro. exact: to_heap_mark_low.
+    - by rewrite low_loc lowloc_eq /lowloc_def.
+  Qed.
+
+  (** Heap rules for high and low locations. *)
+  Lemma wp_alloc p E e v :
+    to_val e = Some v → ↑heapN ⊆ E →
+    {{{ heap_ctx }}} Alloc e @ p; E {{{ l, RET LitV (LitLoc l); l ↦ v }}}.
+  Proof.
+    iIntros (<-%of_to_val ? Φ) "#Hinv HΦ". rewrite /heap_ctx.
+    iMod (auth_empty heap_name) as "Ha".
+    iMod (auth_open with "[$Hinv $Ha]") as ([h h']) "(%&[Hh Hlow]&Hcl)";
+      first done.
+    iApply (wp_alloc_pst with "Hh"); first done. iNext. iIntros (l) "[% Hh]".
+    iDestruct (hinv_high with "Hh Hlow") as "Hh".
+    iMod ("Hcl" with "* [Hh]") as "Ha".
+    - iFrame. iPureIntro. exact: to_heap_alloc_high.
+    - iApply "HΦ". by rewrite mapsto_eq /mapsto_def.
+  Qed.
+
+  Lemma wp_alloc_low p E e v :
+    to_val e = Some v → ↑heapN ⊆ E →
+    {{{ heap_ctx ∗ ▷ low v }}} Alloc e @ p; E
+    {{{ l, RET LitV (LitLoc l); low l }}}.
+  Proof.
+    iIntros (?? Φ) "[#Hinv Hv] HΦ". rewrite -wp_fupd.
+    iApply (wp_alloc with "Hinv"); eauto.
+    iNext. iIntros (l) "Hl". rewrite [(l ↦ v)%I]later_intro [low _]later_intro.
+    iDestruct (heap_mark_low with "Hinv Hl Hv") as "Hl"; first done.
+    by iApply ("HΦ" with "Hl").
+  Qed.
+
+  Lemma wp_load p E l q v :
+    ↑heapN ⊆ E →
+    {{{ heap_ctx ∗ ▷ l ↦{q} v }}} Load (Lit (LitLoc l)) @ p; E
+    {{{ RET v; l ↦{q} v }}}.
+  Proof.
+    iIntros (? Φ) "[#Hinv >Hl] HΦ".
+    rewrite /heap_ctx mapsto_eq /mapsto_def.
+    iMod (auth_open_strong with "[$Hinv $Hl]")
+      as ([h h']) "(%&%&[Hh Hlow]&Hcl)"; first done.
+    case: (to_heap_high_included h h' l q v) => // ??.
+    iApply (wp_load_pst with "Hh"); [done|exact: lookup_union_Some_l|].
+    iNext; iIntros "Hh". iDestruct (hinv_intro with "Hh Hlow") as "Hh".
+    iMod ("Hcl" with "* [Hh]") as "Ha"; first by eauto. by iApply "HΦ".
+  Qed.
+
+  Lemma wp_load_low p E l :
+    ↑heapN ⊆ E →
+    {{{ heap_ctx ∗ ▷ low l }}} Load (Lit (LitLoc l)) @ p; E
+    {{{ v, RET v; low v }}}.
+  Proof.
+    iIntros (? Φ) "[#Hinv >Hl] HΦ".
+    rewrite /heap_ctx low_loc lowloc_eq /lowloc_def.
+    iMod (auth_open_strong with "[$Hinv $Hl]")
+      as ([h h']) "(%&%&[Hh Hlow]&Hcl)"; first done.
+    case: (to_heap_low_included h h' l) => // ? [v ?].
+    iApply (wp_load_pst with "Hh"); [done|exact: lookup_union_Some_r'|].
+    iNext; iIntros "Hh".
+    iDestruct (big_sepM_lookup _ _ l v with "Hlow") as "#Hv"; first done.
+    iDestruct (hinv_intro with "Hh Hlow") as "Hh".
+    iMod ("Hcl" with "* [Hh]") as "Ha"; first by eauto.
+    by iApply ("HΦ" with "Hv").
+  Qed.
+
+  Lemma wp_store p E l v' e v :
+    to_val e = Some v → ↑heapN ⊆ E →
+    {{{ heap_ctx ∗ ▷ l ↦ v' }}} Store (Lit (LitLoc l)) e @ p; E
+    {{{ RET LitV LitUnit; l ↦ v }}}.
+  Proof.
+    iIntros (<-%of_to_val ? Φ) "[#Hinv >Hl] HΦ".
+    rewrite /heap_ctx mapsto_eq /mapsto_def.
+    iMod (auth_open_strong with "[$Hinv $Hl]")
+      as ([h h']) "(%&%&[Hh Hlow]&Hcl)"; first done.
+    case: (to_heap_high_included h h' l 1 v') => // ??.
+    iApply (wp_store_pst with "Hh"); [done|exact: lookup_union_Some_l|].
+    iNext; iIntros "Hh". iDestruct (hinv_high with "Hh Hlow") as "Hh".
+    iMod ("Hcl" with "* [Hh]") as "Ha"; last by iApply "HΦ".
+    iFrame. iPureIntro. exact: to_heap_store_high.
+  Qed.
+
+  Lemma wp_store_low p E l e v :
+    to_val e = Some v → ↑heapN ⊆ E →
+    {{{ heap_ctx ∗ ▷ low  l ∗ ▷ low  v }}} Store (Lit (LitLoc l)) e @ p; E
+    {{{ RET LitV LitUnit; True }}}.
+  Proof.
+    iIntros (<-%of_to_val ? Φ) "(#Hinv&>Hl&Hv) HΦ".
+    rewrite /heap_ctx low_loc lowloc_eq /lowloc_def.
+    iMod (auth_open_strong with "[$Hinv $Hl]")
+      as ([h h']) "(%&%&[Hh Hlow]&Hcl)"; first done.
+    case: (to_heap_low_included h h' l) => // ? [v' ?].
+    iApply (wp_store_pst with "Hh"); [done|exact: lookup_union_Some_r'|].
+    iNext; iIntros "Hh".
+    iDestruct (hinv_store_low with "Hh Hlow Hv") as "Hh"; try done.
+    iMod ("Hcl" with "* [Hh]") as "Ha"; last by iApply "HΦ".
+    iFrame. by erewrite to_heap_low_insert_override.
+  Qed.
+
+  Lemma wp_cas_fail p E l q v' e1 v1 e2 v2 :
+    to_val e1 = Some v1 → to_val e2 = Some v2 → v' ≠ v1 → ↑heapN ⊆ E →
+    {{{ heap_ctx ∗ ▷ l ↦{q} v' }}} CAS (Lit (LitLoc l)) e1 e2 @ p; E
+    {{{ RET LitV (LitBool false); l ↦{q} v' }}}.
+  Proof.
+    iIntros (<-%of_to_val <-%of_to_val ?? Φ) "[#Hinv >Hl] HΦ".
+    rewrite /heap_ctx mapsto_eq /mapsto_def.
+    iMod (auth_open_strong with "[$Hinv $Hl]")
+      as ([h h']) "(%&%&[Hh Hlow]&Hcl)"; first done.
+    case: (to_heap_high_included h h' l q v') => // ??.
+    iApply (wp_cas_fail_pst with "Hh");
+      [done|exact: lookup_union_Some_l|done|].
+    iNext; iIntros "Hh". iDestruct (hinv_intro with "Hh Hlow") as "Hh".
+    iMod ("Hcl" with "* [Hh]") as "Ha"; first eauto. by iApply "HΦ".
+  Qed.
+
+  Lemma wp_cas_suc p E l e1 v1 e2 v2 :
+    to_val e1 = Some v1 → to_val e2 = Some v2 → ↑heapN ⊆ E →
+    {{{ heap_ctx ∗ ▷ l ↦ v1 }}} CAS (Lit (LitLoc l)) e1 e2 @ p; E
+    {{{ RET LitV (LitBool true); l ↦ v2 }}}.
+  Proof.
+    iIntros (<-%of_to_val <-%of_to_val ? Φ) "[#Hinv >Hl] HΦ".
+    rewrite /heap_ctx mapsto_eq /mapsto_def.
+    iMod (auth_open_strong with "[$Hinv $Hl]")
+      as ([h h']) "(%&%&[Hh Hlow]&Hcl)"; first done.
+    case: (to_heap_high_included h h' l 1 v1) => // ??.
+    iApply (wp_cas_suc_pst with "Hh");
+      [done|exact: lookup_union_Some_l|].
+    iNext; iIntros "Hh". iDestruct (hinv_high with "Hh Hlow") as "Hh".
+    iMod ("Hcl" with "* [Hh]") as "Ha"; last by iApply "HΦ".
+    iFrame. iPureIntro. exact: to_heap_store_high.
+  Qed.
+
+  Lemma wp_cas_low p E l e1 v1 e2 v2 :
+    to_val e1 = Some v1 → to_val e2 = Some v2 → ↑heapN ⊆ E →
+    {{{ heap_ctx ∗ ▷ low l ∗ ▷ low v2 }}} CAS (Lit (LitLoc l)) e1 e2 @ p; E
+    {{{ b, RET LitV (LitBool b); True }}}.
+  Proof.
+    iIntros (<-%of_to_val <-%of_to_val ? Φ) "(#Hinv&>Hl&Hv) HΦ".
+    rewrite /heap_ctx low_loc lowloc_eq /lowloc_def.
+    iMod (auth_open_strong with "[$Hinv $Hl]")
+      as ([h h']) "(%&%&[Hh Hlow]&Hcl)"; first done.
+    case: (to_heap_low_included h h' l) => // ? [v' ?].
+    case: (decide (v' = v1)) => [<-|?].
+    - iApply (wp_cas_suc_pst with "Hh");
+        [done|exact: lookup_union_Some_r'|].
+      iNext; iIntros "Hh".
+      iDestruct (hinv_store_low with "Hh Hlow Hv") as "Hh"; try done.
+      iMod ("Hcl" with "* [Hh]") as "Ha"; last by iApply "HΦ".
+      iFrame. by erewrite to_heap_low_insert_override.
+    - iApply (wp_cas_fail_pst with "Hh");
+        [done|exact: lookup_union_Some_r'|done|].
+      iNext; iIntros "Hh". iDestruct (hinv_intro with "Hh Hlow") as "Hh".
+      iMod ("Hcl" with "* [Hh]") as "Ha"; first by eauto. by iApply "HΦ".
+  Qed.
+End heap.
