theories/heap_lang/robust_safety.v
@@ -1,0 +1,1410 @@
+From iris.prelude Require Import countable decidable.
+From iris.base_logic Require Import big_op.
+From iris.heap_lang Require Export heap.
+From iris.heap_lang Require Import addenda proofmode.
+From iris.proofmode Require Import tactics.
+Import addenda.list addenda.fin_maps.
+Import uPred.
+
+Local Hint Resolve to_of_val.
+
+(** * Eliminating low values *)
+(**
+  These lemmas are useful at the boundary between verified and
+  adversarial code.
+*)
+Section wp_low_val.
+  Context `{heapG Σ}.
+  Implicit Types e : expr.
+  Implicit Types v : val.
+
+  Lemma wp_low_val_app v1 v2 :
+    {{{ low v1 ∗ low v2 }}} App (of_val v1) (of_val v2)
+    ?{{{ v, RET v; low v }}}.
+  Proof.
+    iIntros (Φ) "#[Hv1 Hv2] HΦ".
+    case: (decide (is_rec (of_val v1)))=>Hrec;
+      last by iApply wp_stuck_app_nrec.
+    move: Hrec=>[] f [] x [] erec Hrec.
+    case: (decide (Closed (f :b: x :b: []) erec))=>?;
+      last by iApply wp_stuck_app_open.
+    have->: v1 = RecV f x erec.
+    { apply (inj Some). by rewrite -to_val_rec Hrec to_of_val. }
+    rewrite (low_val (RecV _ _ _)) always_elim.
+    iApply wp_rec; [done|by exists v2|]. iNext.
+    iApply (wp_wand with "[] [$HΦ]"). by iApply ("Hv1" with "[$Hv2]").
+  Qed.
+
+  Lemma un_op_eval_low op v1 v2 : un_op_eval op v1 = Some v2 → low v2.
+  Proof.
+    by case: op; case: v1=> // -[] // ? /= [] <-; rewrite low_val low_lit.
+  Qed.
+
+  Lemma wp_low_val_un_op E op v Φ :
+    ▷(∀ v, low v -∗ Φ v) -∗ WP UnOp op (of_val v) @ E ?{{ Φ }}.
+  Proof.
+    iIntros "HΦ".
+    case EV: (un_op_eval op v)=>[v'|]; last by iApply wp_stuck_un_op.
+    wp_op. iApply "HΦ". by iApply un_op_eval_low.
+  Qed.
+
+  Lemma bin_op_eval_low op v1 v2 v3 :
+    bin_op_eval op v1 v2 = Some v3 → low v3.
+  Proof.
+    case: op; try by case: v1=> // -[] // ?; case: v2=>// -[] // ? /= [] <-;
+      rewrite low_val low_lit.
+    by rewrite/bin_op_eval; case: (bool_decide _)=> -[] <-;
+      rewrite low_val low_lit.
+  Qed.
+
+  Lemma wp_low_val_bin_op E op v1 v2 Φ :
+    ▷(∀ v, low v -∗ Φ v) -∗ WP BinOp op (of_val v1) (of_val v2) @ E ?{{ Φ }}.
+  Proof.
+    iIntros "HΦ".
+    case EV: (bin_op_eval op v1 v2)=>[v'|]; last by iApply wp_stuck_bin_op.
+    wp_op. iApply "HΦ". by iApply bin_op_eval_low.
+  Qed.
+
+  Lemma wp_low_val_if E v e1 e2 Φ :
+    ▷ (WP e1 @ E ?{{ Φ }} ∧ WP e2 @ E ?{{ Φ }}) -∗
+    WP If (of_val v) e1 e2 @ E ?{{ Φ }}.
+  Proof.
+    iIntros "Hes".
+    case: (decide (is_lit_bool (of_val v)))=>Hbool; last by iApply wp_stuck_if.
+    case: Hbool=>[] [] <-; wp_if.
+    by iDestruct "Hes" as "[? _]". by iDestruct "Hes" as "[_ ?]".
+  Qed.
+
+  Lemma wp_low_val_fst E v :
+    {{{ low v }}} Fst (of_val v) @ E ?{{{ v, RET v; low v }}}.
+  Proof.
+    iIntros (Φ) "#Hv HΦ".
+    case: (decide (is_pair_val (of_val v)))=>Hp; last by iApply wp_stuck_fst.
+    case: Hp=>e1 [] e2 [] [] v1 He1 [] [] v2 He2 Hp. rewrite Hp.
+    iApply wp_fst; [done|by exists v2|]. have->: v = PairV v1 v2.
+    { move: Hp He1 He2. case: v=> //= v1' v2' [] <-<-.
+      by rewrite 2!to_of_val => -[] -> [] ->. }
+    rewrite low_val. iDestruct "Hv" as "(Hv1&_)". iNext.
+    by iApply ("HΦ" with "[$Hv1]").
+  Qed.
+
+  Lemma wp_low_val_snd E v :
+    {{{ low v }}} Snd (of_val v) @ E ?{{{ v, RET v; low v }}}.
+  Proof.
+    iIntros (Φ) "#Hv HΦ".
+    case: (decide (is_pair_val (of_val v)))=>Hp; last by iApply wp_stuck_snd.
+    case: Hp=>e1 [] e2 [] [] v1 He1 [] [] v2 He2 Hp. rewrite Hp.
+    iApply wp_snd; [by exists v1|done|]. have->: v = PairV v1 v2.
+    { move: Hp He1 He2. case: v=> //= v1' v2' [] <-<-.
+      by rewrite 2!to_of_val => -[] -> [] ->. }
+    rewrite low_val. iDestruct "Hv" as "(_&Hv2)". iNext.
+    by iApply ("HΦ" with "[$Hv2]").
+  Qed.
+
+  Lemma wp_low_val_case E v e1 e2 Φ :
+    low v -∗
+    ▷ (∀ v0, low v0 -∗
+      WP App e1 (of_val v0) @ E ?{{ Φ }} ∧
+      WP App e2 (of_val v0) @ E ?{{ Φ }}) -∗
+    WP Case (of_val v) e1 e2 @ E ?{{ Φ }}.
+  Proof.
+    iIntros "#Hv Hk".
+    case: (decide (is_inj_val (of_val v)))=>Hc; last by iApply wp_stuck_case.
+    move: Hc=>[] e0 [] [] v0 He0 [] Hc; rewrite Hc -(of_to_val e0 v0) //.
+    - iApply wp_case_inl; first by exists v0.
+      have->: v = InjLV v0 by move: Hc He0; case: v => //= v' [] <-;
+        rewrite to_of_val => -[] ->.
+      rewrite low_val. iNext. setoid_rewrite and_elim_l.
+      by iApply ("Hk" with "[$Hv]").
+    - iApply wp_case_inr; first by exists v0.
+      have->: v = InjRV v0 by move: Hc He0; case: v => //= v' [] <-;
+        rewrite to_of_val => -[] ->.
+      rewrite low_val. iNext. setoid_rewrite and_elim_r.
+      by iApply ("Hk" with "[$Hv]").
+  Qed.
+
+  Lemma wp_low_val_load E v :
+    ↑heapN ⊆ E →
+    {{{ heap_ctx ∗ ▷low v }}} Load (of_val v) @ E ?{{{ v, RET v; low v }}}.
+  Proof.
+    iIntros (? Φ) "#(Hh&Hv) HΦ".
+    case: (decide (is_loc (of_val v)))=>Hl; last by iApply wp_stuck_load.
+    case: Hl=>l Hl. rewrite Hl.
+    iApply (wp_load_low with "[$Hh Hv] [$HΦ]"); first done.
+    have->: v = LitV (LitLoc l) by case: v Hl => // -[] //= ? [] ->.
+    rewrite low_val low_lit. by iFrame.
+  Qed.
+
+  Lemma wp_low_val_store E v1 v2 :
+    ↑heapN ⊆ E →
+    {{{ heap_ctx ∗ ▷low v1 ∗ ▷low v2 }}} Store (of_val v1) (of_val v2) @ E
+    ?{{{ v, RET v; low v }}}.
+  Proof.
+    iIntros (? Φ) "(Hh&Hv1&Hv2) HΦ".
+    case: (decide (is_loc (of_val v1)))=>Hl; last by iApply wp_stuck_store.
+    case: Hl=>l Hl. rewrite Hl.
+    iApply (wp_store_low with "[$Hh Hv1 $Hv2] [HΦ]"); [done|done| |].
+    - have->: v1 = LitV (LitLoc l) by case: v1 Hl => // -[] //= ? [] ->.
+      rewrite low_val low_lit. by iFrame.
+    - iNext. iIntros "_". iApply "HΦ". by rewrite low_val low_lit.
+  Qed.
+
+  Lemma wp_low_val_cas E v1 v2 v3 :
+    ↑heapN ⊆ E →
+    {{{ heap_ctx ∗ ▷low v1 ∗ ▷low v3 }}}
+      CAS (of_val v1) (of_val v2) (of_val v3) @ E
+    ?{{{ v, RET v; low v }}}.
+  Proof.
+    iIntros (? Φ) "(Hh&Hv1&Hv3) HΦ".
+    case: (decide (is_loc (of_val v1)))=>Hl; last by iApply wp_stuck_cas.
+    case: Hl=>l Hl. rewrite Hl.
+    iApply (wp_cas_low with "[$Hh Hv1 $Hv3] [HΦ]"); [done|done|done| |].
+    - have->: v1 = LitV (LitLoc l) by case: v1 Hl => // -[] //= ? [] ->.
+      rewrite low_val low_lit. by iFrame.
+    - iNext. iIntros (b) "_". iApply "HΦ". by rewrite low_val low_lit.
+  Qed.
+End wp_low_val.
+
+(** * Substitution of values for binders *)
+Section substitution.
+  Context `{heapG Σ}.
+  Implicit Types e : expr.
+  Implicit Types v : val.
+
+  Definition encode_binder (x : binder) : positive :=
+    encode (if x is BNamed x then Some x else None).
+  Definition decode_binder (p : positive) : option binder :=
+    if decode p is Some opt then
+      Some (if opt is Some x then BNamed x else BAnon)
+    else None.
+  Lemma decode_encode_binder x :
+    decode_binder (encode_binder x) = Some x.
+  Proof.
+    case: x=>[|x]. by naive_solver.
+    by rewrite/encode_binder/decode_binder decode_encode.
+  Qed.
+  Instance binder_countable : Countable binder := {|
+    encode := encode_binder; decode := decode_binder;
+    decode_encode := decode_encode_binder
+  |}.
+
+  Definition env := gmap binder val.
+  Implicit Types Γ : env.
+
+  Definition substitute_acc : binder * val → (expr → expr) → expr → expr :=
+    λ xv f, let: (x, v) := xv in λ e, subst' x (of_val v) (f e).
+  Definition substitute' : list (binder * val) → expr → expr :=
+    foldr substitute_acc id.
+  Definition substitute : env → expr → expr := substitute' ∘ map_to_list.
+
+  Lemma substitute'_cons x v L e :
+    substitute' ((x, v) :: L) e = subst' x (of_val v) (substitute' L e).
+  Proof. by []. Qed.
+
+  Notation ext R := (pointwise_relation _ R).
+  Instance substitute_acc_proper :
+    Proper ((=) ==> ext (=) ==> ext (=)) substitute_acc.
+  Proof.
+    move=>[x v] [??] [<-<-] f1 f2 EQf e. by rewrite/substitute_acc (EQf e).
+  Qed.
+
+  Lemma substitute'_proper L1 L2 :
+    (∀ x v v', (x, v) ∈ L1 → (x, v') ∈ L1 → v = v') →
+    L1 ≡ₚ L2 →
+    ext (=) (substitute' L1) (substitute' L2).
+  Proof.
+    rewrite/substitute'=>Hfun EQ. elim: EQ Hfun=> {L1 L2}.
+    - done.
+    - move=>[x v] L1' L2' EQ IH Hfun.
+      do 2!rewrite foldr_cons. apply substitute_acc_proper, IH.
+      done. by intros; eapply Hfun, elem_of_cons; right.
+    - move=>[x v] [y v'] L Hfun e.
+      do 4!rewrite foldr_cons. rewrite {1 2 4 5}/substitute_acc.
+      case: (decide (x = y))=>?; last by rewrite subst_subst_ne'.
+      subst. do 2!rewrite subst_subst'. do 2!f_equal.
+      eapply Hfun; last by apply elem_of_cons; left.
+      apply elem_of_cons. right. apply elem_of_cons. by left.
+    - move=>L1 L L2 EQ1 IH1 EQ2 IH2 Hfun.
+      rewrite (IH1 Hfun) (IH2 _)=> // x v v' ??.
+      by eapply Hfun; eapply elem_of_list_permutation_proper.
+  Qed.
+
+  Lemma substitute_empty e : e = substitute ∅ e. Proof. by []. Qed.
+
+  Lemma subst_substitute Γ x v e :
+    Γ !! x = None →
+    subst' x (of_val v) (substitute Γ e) = substitute (<[x:=v]>Γ) e.
+  Proof.
+    move=>?. rewrite /substitute/compose -substitute'_cons.
+    symmetry. apply substitute'_proper.
+    exact: map_to_list_unique. by rewrite map_to_list_insert.
+  Qed.
+
+  Lemma substitute_closed Γ e : Closed [] e → substitute Γ e = e.
+  Proof.
+    move=>?. induction Γ as [|x v Γ Hx IH] using map_ind; first done.
+    rewrite -subst_substitute // IH.
+    case: x Hx=> //= x Hx. exact: subst_is_closed_nil.
+  Qed.
+
+  Lemma substitute_expr : ∀ Γ e, let s := substitute Γ in
+    s e =
+    match e with
+    | Var x => default (Var x) (Γ !! BNamed x) of_val
+    | Rec f x e => Rec f x $ substitute (delete f $ delete x $ Γ) e
+    | App e1 e2 => App (s e1) (s e2)
+    | Lit lit => e
+    | UnOp op e => UnOp op (s e)
+    | BinOp op e1 e2 => BinOp op (s e1) (s e2)
+    | If e1 e2 e3 => If (s e1) (s e2) (s e3)
+    | Pair e1 e2 => Pair (s e1) (s e2)
+    | Fst e => Fst (s e)
+    | Snd e => Snd (s e)
+    | InjL e => InjL (s e)
+    | InjR e => InjR (s e)
+    | Case e1 e2 e3 => Case (s e1) (s e2) (s e3)
+    | Assert e => Assert (s e)
+    | Fork e => Fork (s e)
+    | Alloc e => Alloc (s e)
+    | Load e => Load (s e)
+    | Store e1 e2 => Store (s e1) (s e2)
+    | CAS e1 e2 e3 => CAS (s e1) (s e2) (s e3)
+    end.
+  Proof.
+    have nullary: ∀ Γ e, (∀ x es, subst x es e = e) → substitute Γ e = e.
+    { move=>Γ e Hf.
+      have{Hf} Hf: ∀ x es, subst' x es e = e by case.
+      induction Γ as [|x v Γ Hx IH] using map_ind; first done.
+      by rewrite -subst_substitute // IH Hf. }
+    Local Ltac by_induction Γ Hf :=
+      let IH := fresh "IH" in
+      induction Γ as [|x v Γ Hx IH] using map_ind; first done;
+      by rewrite -subst_substitute // IH Hf; f_equal; rewrite subst_substitute.
+    have unary: ∀ f Γ e, (∀ x es e, subst x es (f e) = f (subst x es e)) →
+      substitute Γ (f e) = f (substitute Γ e).
+    { move=>f Γ e Hf.
+      have{Hf} Hf: ∀ x es e, subst' x es (f e) = f (subst' x es e) by case.
+      by_induction Γ Hf. }
+    have binary: ∀ f Γ e1 e2,
+      (∀ x es e1 e2, subst x es (f e1 e2) = f (subst x es e1) (subst x es e2)) →
+      substitute Γ (f e1 e2) = f (substitute Γ e1) (substitute Γ e2).
+    { move=>f Γ e1 e2 Hf.
+      have{Hf} Hf: ∀ x es e1 e2, subst' x es (f e1 e2) =
+         f (subst' x es e1) (subst' x es e2) by case.
+      by_induction Γ Hf. }
+    have ternary: ∀ f Γ e1 e2 e3,
+      (∀ x es e1 e2 e3, subst x es (f e1 e2 e3) =
+       f (subst x es e1) (subst x es e2) (subst x es e3)) →
+      substitute Γ (f e1 e2 e3) =
+      f (substitute Γ e1) (substitute Γ e2) (substitute Γ e3).
+    { move=>f Γ e1 e2 e3 Hf.
+      have{Hf} Hf: ∀ x es e1 e2 e3, subst' x es (f e1 e2 e3) =
+        f (subst' x es e1) (subst' x es e2) (subst' x es e3) by case.
+      by_induction Γ Hf. }
+    move=>Γ /= []; try by auto using nullary, unary, binary, ternary.
+    - move=> x {nullary unary binary ternary}.
+      induction Γ as [|y v Γ Hy IH] using map_ind; first done.
+      rewrite -subst_substitute // IH {IH}. case: (decide (BNamed x = y)) => ?.
+      { subst. by rewrite Hy lookup_insert /= /subst decide_True. }
+      rewrite lookup_insert_ne //. destruct y as [|y]; first done.
+      case: (_ !! _)=>[?|] =>/=.
+      + rewrite subst_is_closed_nil //. exact: is_closed_of_val.
+      + rewrite/subst decide_False // => ?. by subst.
+    - move=>f x e {nullary unary binary ternary}.
+      induction Γ as [|y v Γ Hy IH] using map_ind; first done.
+      rewrite -subst_substitute // IH {IH}.
+      case: (decide (y ≠ f ∧ y ≠ x))=>[[??]| /not_and_l EQ].
+      { rewrite subst_rec_ne'; [| by left | by left]. f_equal.
+        rewrite subst_substitute; last by do 2!rewrite lookup_delete_ne //.
+        by do 2!rewrite delete_insert_ne //. }
+      rewrite subst_rec'; last by case: EQ=>/dec_stable; [left| right; left].
+      do 2!f_equal. case: EQ=>/dec_stable ?; subst.
+      + by rewrite delete_commute [delete f _]delete_notin //
+          delete_commute delete_insert //.
+      + f_equal. by rewrite delete_notin // delete_insert //.
+  Qed.
+End substitution.
+
+(** * The fundamental theorem of logical relations *)
+(**
+	We model adversarial values and closed, adversarial
+	expressions with [low v] and [WP e ?{{ low }}], respectively
+	(see [low_val]). Our aim is to show that, under the heap
+	invariant, all syntactically low expressions (see [low_expr])
+	inhabit the model.
+
+	The proof is by induction on expressions. For the induction to
+	go through, we must generalize to account for substitution of
+	low values for variables. (Since the expression relation does
+	not imply progress, these need not be closing substitutions.)
+ *)
+Section ftlr.
+
+  Context `{heapG Σ}.
+  Implicit Types Γ : env.
+  Implicit Types e : expr.
+  Implicit Types v : val.
+
+  Instance env_low : LowIntegrity Σ env := Low (λ Γ, [∗ map] v ∈ Γ, low v)%I _.
+
+  Definition confined : expr → iProp Σ := λ e, (
+    ∀ Γ, heap_ctx -∗ low Γ -∗ low e -∗ WP substitute Γ e ?{{ low }}
+  )%I.
+
+  Lemma low_env Γ : low Γ ⊣⊢ [∗ map] v ∈ Γ, low v. Proof. by []. Qed.
+
+  Lemma low_env_empty : low (∅ : env) ⊣⊢ True.
+  Proof. exact: big_sepM_empty. Qed.
+
+  Lemma low_env_insert Γ x v :
+    Γ !! x = None → low v -∗ low Γ -∗ low (<[x:=v]>Γ).
+  Proof.
+    do 2!rewrite low_env. move=>?. rewrite big_sepM_insert //.
+    iIntros. by iFrame "#".
+  Qed.
+
+  Lemma low_env_singleton x v : low ({[x:=v]} : env) ⊣⊢ low v.
+  Proof. exact: big_sepM_singleton. Qed.
+
+  Lemma low_env_lookup Γ x v : Γ !! x = Some v → low Γ -∗ low v.
+  Proof. exact: big_sepM_lookup. Qed.
+
+  Lemma low_env_delete Γ x  : low Γ -∗ low (delete x Γ).
+  Proof.
+    rewrite low_env. apply big_sepM_mono. exact: delete_subseteq. done.
+  Qed.
+
+  Lemma confined_alt e :
+    confined e ⊣⊢
+    ∀ Γ Φ, heap_ctx -∗ low Γ -∗ low e -∗ (∀ v, low v -∗ Φ v) -∗
+    WP substitute Γ e ?{{ Φ }}.
+  Proof.
+    iSplit.
+    - iIntros "Hc". iIntros (Γ Φ) "Hh HΓ He". rewrite -wp_wand.
+      by iApply ("Hc" with "[$Hh] [$HΓ] [$He]").
+    - iIntros "Halt". iIntros (Γ) "Hh HΓ He".
+      iApply ("Halt" with "[$Hh] [$HΓ] [$He] []"). by iIntros.
+  Qed.
+
+  Lemma confined_var x : confined (Var x).
+  Proof.
+    iIntros (Γ) "_ #HΓ _". rewrite substitute_expr.
+    case Hdom: (_ !! _)=>[v|]/=; last by iApply wp_stuck_var.
+    iApply wp_value'. by iApply (low_env_lookup with "[$HΓ]").
+  Qed.
+
+  Lemma of_val_rec f x e `{!Closed (f :b: x :b: []) e} :
+    Rec f x e = of_val (RecV f x e).
+  Proof. symmetry. apply of_to_val. exact: to_val_rec. Qed.
+
+  Lemma confined_rec f x e : (□ confined e) -∗ confined (Rec f x e).
+  Proof.
+    iIntros "#IHe". iIntros (Γ) "#Hh #HΓ #He".
+    rewrite low_expr substitute_expr. set erec := substitute _ _.
+    case: (decide (Closed (f :b: x :b: []) erec)) => ?;
+      last by iApply wp_stuck_rec_open.
+    iApply wp_value; first exact: to_val_rec.
+    rewrite/erec. set Γ' := (delete _ _).
+    iLöb as "Hvrec". rewrite {2}low_val. iAlways. iNext.
+    iIntros (v2) "#Hv2". case: (decide (x = f))=>?.
+    { subst. rewrite -> subst_subst'; last done.	(* ssr rewrite fails *)
+      rewrite of_val_rec subst_substitute; last by rewrite lookup_delete.
+      iApply ("IHe" with "[$Hh] [] [$He]").
+      rewrite insert_delete. iApply (low_env_insert with "[$Hvrec] []");
+        first by rewrite lookup_delete.
+      by iApply (low_env_delete with "[$HΓ]"). }
+    rewrite of_val_rec subst_substitute; last by rewrite lookup_delete.
+    rewrite subst_substitute; last by rewrite
+      lookup_insert_ne // lookup_delete_ne // lookup_delete.
+    iApply ("IHe" with "[$Hh] [] [$He]").
+    iApply (low_env_insert with "[$Hv2] []"); first by rewrite
+      lookup_insert_ne // lookup_delete_ne // lookup_delete.
+    iApply (low_env_insert with "[$Hvrec] []"); first by rewrite
+      lookup_delete.
+    do 2!iApply low_env_delete. iExact "HΓ".
+  Qed.
+
+  Lemma confined_app e1 e2 : confined e1 -∗ confined e2 -∗ confined (App e1 e2).
+  Proof.
+    rewrite (confined_alt (App _ _)).
+    iIntros "IHe1 IHe2". iIntros (Γ Φ) "#Hh #HΓ Happ HΦ".
+    rewrite low_expr substitute_expr. iDestruct "Happ" as "(He1&He2)".
+    wp_bind (substitute _ _). rewrite confined_alt.
+    iApply ("IHe1" with "[$Hh] [$HΓ] [$He1]"). iIntros (v1) "Hv1".
+    wp_bind (substitute _ _). rewrite confined_alt.
+    iApply ("IHe2" with "[$Hh] [$HΓ] [$He2]"). iIntros (v2) "Hv2".
+    by iApply (wp_low_val_app with "[$Hv1 $Hv2] [$HΦ]").
+  Qed.
+
+  Lemma confined_lit lit : confined (Lit lit).
+  Proof.
+    iIntros (Γ) "_ _ #?". rewrite low_expr substitute_expr.
+    iApply wp_value; first done. by rewrite low_val.
+  Qed.
+
+  Lemma confined_un_op op e : confined e -∗ confined (UnOp op e).
+  Proof.
+    rewrite (confined_alt (UnOp _ _)).
+    iIntros "IHe". iIntros (Γ Φ) "Hh HΓ He HΦ".
+    rewrite low_expr substitute_expr.
+    wp_bind (substitute _ _). rewrite confined_alt.
+    iApply ("IHe" with "[$Hh] [$HΓ] [$He]"). iIntros (v) "_".
+    by iApply (wp_low_val_un_op with "[$HΦ]").
+  Qed.
+
+  Lemma confined_bin_op op e1 e2 :
+    confined e1 -∗ confined e2 -∗ confined (BinOp op e1 e2).
+  Proof.
+    rewrite (confined_alt (BinOp _ _ _)).
+    iIntros "IHe1 IHe2". iIntros (Γ Φ) "#Hh #HΓ Hop HΦ".
+    rewrite low_expr substitute_expr. iDestruct "Hop" as "(He1&He2)".
+    wp_bind (substitute _ _). rewrite confined_alt.
+    iApply ("IHe1" with "[$Hh] [$HΓ] [$He1]"). iIntros (v1) "_".
+    wp_bind (substitute _ _). rewrite confined_alt.
+    iApply ("IHe2" with "[$Hh] [$HΓ] [$He2]"). iIntros (v2) "_".
+    by iApply (wp_low_val_bin_op with "[$HΦ]").
+  Qed.
+
+  Lemma confined_if e e1 e2 :
+    confined e -∗ confined e1 -∗ confined e2 -∗ confined (If e e1 e2).
+  Proof.
+    rewrite (confined_alt (If _ _ _)).
+    iIntros "IHe IHe1 IHe2". iIntros (Γ Φ) "#Hh #HΓ Hif HΦ".
+    rewrite low_expr substitute_expr. iDestruct "Hif" as "(He&He1&He2)".
+    wp_bind (substitute _ _). rewrite confined_alt.
+    iApply ("IHe" with "[$Hh] [$HΓ] [$He]"). iIntros (v) "_".
+    iApply wp_low_val_if. iNext. iSplit.
+    - rewrite confined_alt.
+      by iApply ("IHe1" with "[$Hh] [$HΓ] [$He1] [$HΦ]").
+    - rewrite (confined_alt e2).
+      by iApply ("IHe2" with "[$Hh] [$HΓ] [$He2] [$HΦ]").
+  Qed.
+
+  Lemma confined_pair e1 e2 :
+    confined e1 -∗ confined e2 -∗ confined (Pair e1 e2).
+  Proof.
+    rewrite (confined_alt (Pair _ _)).
+    iIntros "IHe1 IHe2". iIntros (Γ Φ) "#Hh #HΓ Hp HΦ".
+    rewrite low_expr substitute_expr. iDestruct "Hp" as "(He1&He2)".
+    wp_bind (substitute _ _). rewrite confined_alt.
+    iApply ("IHe1" with "[$Hh] [$HΓ] [$He1]"). iIntros (v1) "Hv1".
+    wp_bind (substitute _ _). rewrite confined_alt.
+    iApply ("IHe2" with "[$Hh] [$HΓ] [$He2]"). iIntros (v2) "Hv2".
+    iApply wp_value; first by rewrite /= (to_of_val v1) (to_of_val v2).
+    iApply "HΦ". rewrite (low_val (PairV _ _)). by iFrame.
+  Qed.
+
+  Lemma confined_fst e : confined e -∗ confined (Fst e).
+  Proof.
+    rewrite (confined_alt (Fst _)).
+    iIntros "IHe". iIntros (Γ Φ) "#Hh #HΓ He HΦ".
+    rewrite low_expr substitute_expr.
+    wp_bind (substitute _ _). rewrite confined_alt.
+    iApply ("IHe" with "[$Hh] [$HΓ] [$He]"). iIntros (v) "Hv".
+    by iApply (wp_low_val_fst with "[$Hv] [$HΦ]").
+  Qed.
+
+  Lemma confined_snd e : confined e -∗ confined (Snd e).
+  Proof.
+    rewrite (confined_alt (Snd _)).
+    iIntros "IHe". iIntros (Γ Φ) "#Hh #HΓ He HΦ".
+    rewrite low_expr substitute_expr.
+    wp_bind (substitute _ _). rewrite confined_alt.
+    iApply ("IHe" with "[$Hh] [$HΓ] [$He]"). iIntros (v) "Hv".
+    by iApply (wp_low_val_snd with "[$Hv] [$HΦ]").
+  Qed.
+
+  Lemma confined_inl e : confined e -∗ confined (InjL e).
+  Proof.
+    rewrite (confined_alt (InjL _)).
+    iIntros "IHe". iIntros (Γ Φ) "#Hh #HΓ He HΦ".
+    rewrite low_expr substitute_expr.
+    wp_bind (substitute _ _). rewrite confined_alt.
+    iApply ("IHe" with "[$Hh] [$HΓ] [$He]"). iIntros (v) "Hv".
+    iApply wp_value; first by rewrite /= (to_of_val v).
+    iApply "HΦ". rewrite (low_val (InjLV _)). by iFrame.
+  Qed.
+
+  Lemma confined_inr e : confined e -∗ confined (InjR e).
+  Proof.
+    rewrite (confined_alt (InjR _)).
+    iIntros "IHe". iIntros (Γ Φ) "#Hh #HΓ He HΦ".
+    rewrite low_expr substitute_expr.
+    wp_bind (substitute _ _). rewrite confined_alt.
+    iApply ("IHe" with "[$Hh] [$HΓ] [$He]"). iIntros (v) "Hv".
+    iApply wp_value; first by rewrite /= (to_of_val v).
+    iApply "HΦ". rewrite (low_val (InjRV _)). by iFrame.
+  Qed.
+
+  Lemma confined_case e e1 e2 :
+    confined e -∗ confined e1 -∗ confined e2 -∗ confined (Case e e1 e2).
+  Proof.
+    rewrite (confined_alt (Case _ _ _)).
+    iIntros "IHe IHe1 IHe2". iIntros (Γ Φ) "#Hh #HΓ Hc HΦ".
+    rewrite low_expr substitute_expr. iDestruct "Hc" as "(He&He1&He2)".
+    wp_bind (substitute _ _). rewrite confined_alt.
+    iApply ("IHe" with "[$Hh] [$HΓ] [$He]"). iIntros (v) "Hv".
+    iApply (wp_low_val_case with "[$Hv]"). iNext. iIntros (v0) "#Hv0". iSplit.
+    - wp_bind (substitute _ _). rewrite confined_alt.
+      iApply ("IHe1" with "[$Hh] [$HΓ] [$He1]"). iIntros (v1) "Hv1".
+      by iApply (wp_low_val_app with "[$Hv1 $Hv0] [$HΦ]").
+    - wp_bind (substitute _ _). rewrite (confined_alt e2).
+      iApply ("IHe2" with "[$Hh] [$HΓ] [$He2]"). iIntros (v2) "Hv2".
+      by iApply (wp_low_val_app with "[$Hv2 $Hv0] [$HΦ]").
+  Qed.
+
+  Lemma confined_assert e : confined (Assert e).
+  Proof. iIntros (Γ) "_ _ He". rewrite low_expr. by iExFalso. Qed.
+
+  Lemma confined_fork e : confined e -∗ confined (Fork e).
+  Proof.
+    iIntros "IHe". iIntros (Γ) "#Hh #HΓ He".
+    rewrite low_expr substitute_expr. iApply wp_fork. iNext. iSplit.
+    - by rewrite low_val low_lit.
+    - rewrite confined_alt.
+      iApply ("IHe" with "[$Hh] [$HΓ] [$He] []"). by iIntros.
+  Qed.
+
+  Lemma confined_alloc e : confined e -∗ confined (Alloc e).
+  Proof.
+    rewrite (confined_alt (Alloc _)).
+    iIntros "IHe". iIntros (Γ Φ) "#Hh #HΓ He HΦ".
+    rewrite low_expr substitute_expr.
+    wp_bind (substitute _ _). rewrite confined_alt.
+    iApply ("IHe" with "[$Hh] [$HΓ] [$He]"). iIntros (v) "Hv".
+    iApply (wp_alloc_low with "[$Hh $Hv]"); [by rewrite to_of_val|done|].
+    iNext. iIntros (l) "#Hl". iApply "HΦ". by rewrite low_val low_lit.
+  Qed.
+
+  Lemma confined_load e : confined e -∗ confined (Load e).
+  Proof.
+    rewrite (confined_alt (Load _)).
+    iIntros "IHe". iIntros (Γ Φ) "#Hh #HΓ He HΦ".
+    rewrite low_expr substitute_expr.
+    wp_bind (substitute _ _). rewrite confined_alt.
+    iApply ("IHe" with "[$Hh] [$HΓ] [$He]"). iIntros (v) "Hv".
+    by iApply (wp_low_val_load with "[$Hh $Hv] [$HΦ]").
+  Qed.
+
+  Lemma confined_store e1 e2 :
+    confined e1 -∗ confined e2 -∗ confined (Store e1 e2).
+  Proof.
+    rewrite (confined_alt (Store _ _)).
+    iIntros "IHe1 IHe2". iIntros (Γ Φ) "#Hh #HΓ Hstore HΦ".
+    rewrite low_expr substitute_expr. iDestruct "Hstore" as "(He1&He2)".
+    wp_bind (substitute _ _). rewrite confined_alt.
+    iApply ("IHe1" with "[$Hh] [$HΓ] [$He1]"). iIntros (v1) "Hv1".
+    wp_bind (substitute _ _). rewrite confined_alt.
+    iApply ("IHe2" with "[$Hh] [$HΓ] [$He2]"). iIntros (v2) "Hv2".
+    by iApply (wp_low_val_store with "[$Hh $Hv1 $Hv2] [$HΦ]").
+  Qed.
+
+  Lemma confined_cas e0 e1 e2 :
+    confined e0 -∗ confined e1 -∗ confined e2 -∗ confined (CAS e0 e1 e2).
+  Proof.
+    rewrite (confined_alt (CAS _ _ _)).
+    iIntros "IHe0 IHe1 IHe2". iIntros (Γ Φ) "#Hh #HΓ Hcas HΦ".
+    rewrite low_expr substitute_expr. iDestruct "Hcas" as "(He0&He1&He2)".
+    wp_bind (substitute _ _). rewrite confined_alt.
+    iApply ("IHe0" with "[$Hh] [$HΓ] [$He0]"). iIntros (v0) "Hv0".
+    wp_bind (substitute _ _). rewrite confined_alt.
+    iApply ("IHe1" with "[$Hh] [$HΓ] [$He1]"). iIntros (v1) "_".
+    wp_bind (substitute _ _). rewrite confined_alt.
+    iApply ("IHe2" with "[$Hh] [$HΓ] [$He2]"). iIntros (v2) "Hv2".
+    by iApply (wp_low_val_cas with "[$Hh $Hv0 $Hv2] [$HΦ]").
+  Qed.
+
+  Theorem ftlr' e : confined e.
+  Proof.
+    iStartProof. (* iLöb as "IH" forall (e). *)
+    iInduction e as [| | | | | | | | | | | | | | | | | |] "IHe".
+    - by rewrite -confined_var.
+    - by rewrite -confined_rec.
+    - by iRevert "IHe1"; rewrite always_elim -confined_app.
+    - by rewrite -confined_lit.
+    - by rewrite -confined_un_op.
+    - by iRevert "IHe1"; rewrite always_elim -confined_bin_op.
+    - by iRevert "IHe1 IHe2"; rewrite 2!always_elim -confined_if.
+    - by iRevert "IHe1"; rewrite always_elim -confined_pair.
+    - by rewrite -confined_fst.
+    - by rewrite -confined_snd.
+    - by rewrite -confined_inl.
+    - by rewrite -confined_inr.
+    - by iRevert "IHe1 IHe2"; rewrite 2!always_elim -confined_case.
+    - by rewrite -confined_assert.
+    - by rewrite -confined_fork.
+    - by rewrite -confined_alloc.
+    - by rewrite -confined_load.
+    - by iRevert "IHe1"; rewrite always_elim -confined_store.
+    - by iRevert "IHe1 IHe2"; rewrite 2!always_elim -confined_cas.
+  Qed.
+
+  Corollary ftlr e Γ e' Φ :
+    e = substitute Γ e' →
+    heap_ctx -∗ low Γ -∗ low e' -∗ (∀ v, low v -∗ Φ v) -∗ WP e ?{{ Φ }}.
+  Proof.
+    iIntros (->) "Hh HΓ He". rewrite -wp_wand.
+    iApply (ftlr' with "[$Hh] [$HΓ] [$He]").
+  Qed.
+End ftlr.
+
+(** * Contexts *)
+(**
+  Contexts are expressions with a single hole. The following
+  definition must agree with [heap_lang.expr].
+ *)
+Inductive ctx :=
+  | CHole
+  | CRec of binder & binder & ctx
+  | CAppL of ctx & expr
+  | CAppR of expr & ctx
+  | CUnOp of un_op & ctx
+  | CBinOpL of bin_op & ctx & expr
+  | CBinOpR of bin_op & expr & ctx
+  | CIf of ctx & expr & expr
+  | CIfL of expr & ctx & expr
+  | CIfR of expr & expr & ctx
+  | CPairL of ctx & expr
+  | CPairR of expr & ctx
+  | CFst of ctx
+  | CSnd of ctx
+  | CInjL of ctx
+  | CInjR of ctx
+  | CCase of ctx & expr & expr
+  | CCaseL of expr & ctx & expr
+  | CCaseR of expr & expr & ctx
+  | CAssert of ctx
+  | CFork of ctx
+  | CAlloc of ctx
+  | CLoad of ctx
+  | CStoreL of ctx & expr
+  | CStoreR of expr & ctx
+  | CCASL of ctx & expr & expr
+  | CCASM of expr & ctx & expr
+  | CCASR of expr & expr & ctx.
+
+Fixpoint ctx_fill (C : ctx) (e : expr) : expr :=
+  let rec := λ C, ctx_fill C e in
+  match C with
+  | CHole => e
+  | CRec f x C => Rec f x (rec C)
+  | CAppL C1 e2 => App (rec C1) e2
+  | CAppR e1 C2 => App e1 (rec C2)
+  | CUnOp op C => UnOp op (rec C)
+  | CBinOpL op C1 e2 => BinOp op (rec C1) e2
+  | CBinOpR op e1 C2 => BinOp op e1 (rec C2)
+  | CIf C0 e1 e2 => If (rec C0) e1 e2
+  | CIfL e0 C1 e2 => If e0 (rec C1) e2
+  | CIfR e0 e1 C2 => If e0 e1 (rec C2)
+  | CPairL C1 e2 => Pair (rec C1) e2
+  | CPairR e1 C2 => Pair e1 (rec C2)
+  | CFst C => Fst (rec C)
+  | CSnd C => Snd (rec C)
+  | CInjL C => InjL (rec C)
+  | CInjR C => InjR (rec C)
+  | CCase C0 e1 e2 => Case (rec C0) e1 e2
+  | CCaseL e0 C1 e2 => Case e0 (rec C1) e2
+  | CCaseR e0 e1 C2 => Case e0 e1 (rec C2)
+  | CAssert C => Assert (rec C)
+  | CFork C => Fork (rec C)
+  | CAlloc C => Alloc (rec C)
+  | CLoad C => Load (rec C)
+  | CStoreL C1 e2 => Store (rec C1) e2
+  | CStoreR e1 C2 => Store e1 (rec C2)
+  | CCASL C0 e1 e2 => CAS (rec C0) e1 e2
+  | CCASM e0 C1 e2 => CAS e0 (rec C1) e2
+  | CCASR e0 e1 C2 => CAS e0 e1 (rec C2)
+  end.
+
+(**
+	A (syntactically) low context contains neither assertions nor
+	high locations. (We reserve assertions for verified code.)
+*)
+Section low_ctx.
+  Context `{heapG Σ}.
+  Implicit Types C : ctx.
+
+  Definition lowctx : ctx → iProp Σ :=
+    fix rec C := match C with
+    | CHole => True
+    | CAssert _ => False
+    | CRec _ _ C | CUnOp _ C | CFst C | CSnd C | CInjL C | CInjR C
+    | CFork C | CAlloc C | CLoad C
+      => rec C
+    | CAppL C1 e2 | CBinOpL _ C1 e2 | CPairL C1 e2 | CStoreL C1 e2
+      => rec C1 ∗ low e2
+    | CAppR e1 C2 | CBinOpR _ e1 C2 | CPairR e1 C2 | CStoreR e1 C2
+      => low e1 ∗ rec C2
+    | CIf C0 e1 e2 | CCase C0 e1 e2 | CCASL C0 e1 e2
+      => rec C0 ∗ low e1 ∗ low e2
+    | CIfL e0 C1 e2 | CCaseL e0 C1 e2 | CCASM e0 C1 e2
+      => low e0 ∗ rec C1 ∗ low e2
+    | CIfR e0 e1 C2 | CCaseR e0 e1 C2 | CCASR e0 e1 C2
+      => low e0 ∗ low e1 ∗ rec C2
+    end%I.
+  Global Instance lowctx_persistent C : PersistentP (lowctx C).
+  Proof. rewrite/lowctx; elim: C=>//; rewrite-/lowctx; by apply _. Qed.
+  Global Instance lowctx_low : LowIntegrity Σ ctx := Low lowctx _.
+  Global Instance lowctx_timeless (C : ctx) : TimelessP (low C).
+  Proof. rewrite/lowctx; elim: C=>//; rewrite-/lowctx; by apply _. Qed.
+
+  Lemma low_ctx C :
+    low C ⊣⊢
+    match C with
+    | CHole => True
+    | CAssert _ => False
+    | CRec _ _ C | CUnOp _ C | CFst C | CSnd C | CInjL C | CInjR C
+    | CFork C | CAlloc C | CLoad C
+      => low C
+    | CAppL C1 e2 | CBinOpL _ C1 e2 | CPairL C1 e2 | CStoreL C1 e2
+      => low C1 ∗ low e2
+    | CAppR e1 C2 | CBinOpR _ e1 C2 | CPairR e1 C2 | CStoreR e1 C2
+      => low e1 ∗ low C2
+    | CIf C0 e1 e2 | CCase C0 e1 e2 | CCASL C0 e1 e2
+      => low C0 ∗ low e1 ∗ low e2
+    | CIfL e0 C1 e2 | CCaseL e0 C1 e2 | CCASM e0 C1 e2
+      => low e0 ∗ low C1 ∗ low e2
+    | CIfR e0 e1 C2 | CCaseR e0 e1 C2 | CCASR e0 e1 C2
+      => low e0 ∗ low e1 ∗ low C2
+    end%I.
+  Proof. by case: C. Qed.
+End low_ctx.
+
+(** Sanity check. *)
+(**
+	To catch changes to [expr] that aren't reflected in [ctx], we
+	embed evaluation contexts in contexts and prove the filling
+	functions match up.
+*)
+Local Notation ectx := (list ectx_item).
+
+Definition of_ectx_item (Ki : ectx_item) (C : ctx) : ctx :=
+  match Ki with
+  | AppLCtx e2 => CAppL C e2
+  | AppRCtx v1 => CAppR (of_val v1) C
+  | UnOpCtx op => CUnOp op C
+  | BinOpLCtx op e2 => CBinOpL op C e2
+  | BinOpRCtx op v1 => CBinOpR op (of_val v1) C
+  | IfCtx e1 e2 => CIf C e1 e2
+  | PairLCtx e2 => CPairL C e2
+  | PairRCtx v1 => CPairR (of_val v1) C
+  | FstCtx => CFst C
+  | SndCtx => CSnd C
+  | InjLCtx => CInjL C
+  | InjRCtx => CInjR C
+  | CaseCtx e1 e2 => CCase C e1 e2
+  | AssertCtx => CAssert C
+  | AllocCtx => CAlloc C
+  | LoadCtx => CLoad C
+  | StoreLCtx e2 => CStoreL C e2
+  | StoreRCtx v1 => CStoreR (of_val v1) C
+  | CasLCtx e1 e2 => CCASL C e1 e2
+  | CasMCtx v0 e2 => CCASM (of_val v0) C e2
+  | CasRCtx v0 v1 => CCASR (of_val v0) (of_val v1) C
+  end.
+
+Definition of_ectx : ectx → ctx := foldr of_ectx_item CHole.
+
+Fixpoint to_ectx (C : ctx) : option ectx :=
+  let rec := λ C Ki, K ← to_ectx C; Some (Ki :: K) in
+  let recv := λ e C f, v ← to_val e; rec C $ f v in
+  match C with
+  | CHole => Some []
+  | CAppL C e2 => rec C $ AppLCtx e2
+  | CAppR e1 C => recv e1 C $ AppRCtx
+  | CUnOp op C => rec C $ UnOpCtx op
+  | CBinOpL op C e2 => rec C $ BinOpLCtx op e2
+  | CBinOpR op e1 C => recv e1 C $ BinOpRCtx op
+  | CIf C e1 e2 => rec C $ IfCtx e1 e2
+  | CPairL C e2 => rec C $ PairLCtx e2
+  | CPairR e1 C => recv e1 C PairRCtx
+  | CFst C => rec C FstCtx
+  | CSnd C => rec C SndCtx
+  | CInjL C => rec C InjLCtx
+  | CInjR C => rec C InjRCtx
+  | CCase C e1 e2 => rec C $ CaseCtx e1 e2
+  | CAssert C => rec C AssertCtx
+  | CAlloc C => rec C AllocCtx
+  | CLoad C => rec C LoadCtx
+  | CStoreL C e2 => rec C $ StoreLCtx e2
+  | CStoreR e1 C => recv e1 C StoreRCtx
+  | CCASL C e1 e2 => rec C $ CasLCtx e1 e2
+  | CCASM e0 C e2 => v0 ← to_val e0; rec C $ CasMCtx v0 e2
+  | CCASR e0 e1 C => v0 ← to_val e0; v1 ← to_val e1; rec C $ CasRCtx v0 v1
+  | _ => None
+  end.
+
+Lemma to_of_ectx K : to_ectx (of_ectx K) = Some K.
+Proof.
+  elim: K => // Ki K IH. by destruct Ki; simplify_option_eq; repeat f_equal.
+Qed.
+
+Lemma of_to_ectx C K : to_ectx C = Some K → of_ectx K = C.
+Proof.
+  elim: C K; intros; simplify_option_eq; auto using of_to_val with f_equal.
+Qed.
+
+Instance of_ectx_inj : Inj (=) (=) of_ectx.
+Proof. move=>?? EQ. apply (inj Some). by rewrite -!to_of_ectx EQ. Qed.
+
+Lemma to_ectx_fill C K e : to_ectx C = Some K → ctx_fill C e = fill K e.
+Proof.
+  elim: C K; intros; simplify_option_eq;
+    auto using of_to_val, eq_sym with f_equal.
+Qed.
+
+(** * Adversaries *)
+(**
+	To state the [robust_safety] theorem, we define a special case
+	of [low_ctx] at the meta-level. An _adversarial context_ is a
+	heap language context containing neither locations nor
+	assertions.
+*)
+Definition adv_lit : base_lit → Prop :=
+  λ lit, match lit with
+  | LitInt _ | LitBool _ | LitUnit => True
+  | LitLoc _ => False
+  end.
+
+Definition adv_expr : expr → Prop :=
+  fix rec e := match e with
+  | Var _ => True
+  | Assert _ => False
+  | Lit lit => adv_lit lit
+  | Rec _ _ e | UnOp _ e | Fst e | Snd e | InjL e | InjR e
+  | Fork e | Alloc e | Load e
+    => rec e
+  | App e1 e2 | BinOp _ e1 e2 | Pair e1 e2 | Store e1 e2 => rec e1 ∧ rec e2
+  | If e1 e2 e3 | Case e1 e2 e3 | CAS e1 e2 e3
+    => rec e1 ∧ rec e2 ∧ rec e3
+  end.
+
+Definition adv_ctx : ctx → Prop :=
+  fix rec C := match C with
+  | CHole => True
+  | CAssert _ => False
+  | CRec _ _ C | CUnOp _ C | CFst C | CSnd C | CInjL C | CInjR C
+  | CFork C | CAlloc C | CLoad C
+    => rec C
+  | CAppL C1 e2 | CBinOpL _ C1 e2 | CPairL C1 e2 | CStoreL C1 e2
+    => rec C1 ∧ adv_expr e2
+  | CAppR e1 C2 | CBinOpR _ e1 C2 | CPairR e1 C2 | CStoreR e1 C2
+    => adv_expr e1 ∧ rec C2
+  | CIf C0 e1 e2 | CCase C0 e1 e2 | CCASL C0 e1 e2
+    => rec C0 ∧ adv_expr e1 ∧ adv_expr e2
+  | CIfL e0 C1 e2 | CCaseL e0 C1 e2 | CCASM e0 C1 e2
+    => adv_expr e0 ∧ rec C1 ∧ adv_expr e2
+  | CIfR e0 e1 C2 | CCaseR e0 e1 C2 | CCASR e0 e1 C2
+    => adv_expr e0 ∧ adv_expr e1 ∧ rec C2
+  end.
+
+Section adversary.
+    Context `{heapG Σ}.
+  Implicit Types C : ctx.
+  Implicit Types e : expr.
+
+  Lemma adv_lit_low lit : adv_lit lit → low lit.
+  Proof. by case: lit. Qed.
+
+  Lemma adv_expr_low e : adv_expr e → low e.
+  Proof.	(* PDS: Automate. *)
+    elim: e => //.
+    - move=>e1 IH1 e2 IH2 [] ??. rewrite low_expr /=.
+      iIntros. iSplit. by iApply IH1. by iApply IH2.
+    - exact: adv_lit_low.
+    - move=>op e1 IH1 e2 IH2 [] ??. rewrite low_expr /=.
+      iIntros. iSplit. by iApply IH1. by iApply IH2.
+    - move=>e0 IH0 e1 IH1 e2 IH2 [] ? [] ?. rewrite low_expr /=.
+      iIntros. iSplit; last iSplit. by iApply IH0. by iApply IH1. by iApply IH2.
+    - move=>e1 IH1 e2 IH2 [] ??. rewrite low_expr /=.
+      iIntros. iSplit. by iApply IH1. by iApply IH2.
+    - move=>e0 IH0 e1 IH1 e2 IH2 [] ? [] ?. rewrite low_expr /=.
+      iIntros. iSplit; last iSplit. by iApply IH0. by iApply IH1. by iApply IH2.
+    - move=>e1 IH1 e2 IH2 [] ??. rewrite low_expr /=.
+      iIntros. iSplit. by iApply IH1. by iApply IH2.
+    - move=>e0 IH0 e1 IH1 e2 IH2 [] ? [] ?. rewrite low_expr /=.
+      iIntros. iSplit; last iSplit. by iApply IH0. by iApply IH1. by iApply IH2.
+  Qed.
+
+  Lemma adv_ctx_low C : adv_ctx C → low C.
+  Proof.	(* PDS: Automate. *)
+    elim: C => //=.
+    (* application *)
+    - move=>C1 IH e2 [] ??. rewrite low_ctx.
+      iSplit. by iApply IH. by iApply adv_expr_low.
+    - move=>e1 C2 IH [] ??. rewrite low_ctx.
+      iSplit. by iApply adv_expr_low. by iApply IH.
+    (* binary operations *)
+    - move=>op C1 IH e2 [] ??. rewrite low_ctx.
+      iSplit. by iApply IH. by iApply adv_expr_low.
+    - move=>op e1 C2 IH [] ??. rewrite low_ctx.
+      iSplit. by iApply adv_expr_low. by iApply IH.
+    (* if *)
+    - move=>C0 IH e1 e2 [] ? [] ??. rewrite low_ctx.
+      iSplit; [|iSplit]. by iApply IH. by iApply adv_expr_low.
+      by iApply adv_expr_low.
+    - move=>e0 C1 IH e2 [] ? [] ??. rewrite low_ctx.
+      iSplit; [|iSplit]. by iApply adv_expr_low. by iApply IH.
+      by iApply adv_expr_low.
+    - move=>e0 e1 C2 IH [] ? [] ??. rewrite low_ctx.
+      iSplit; [|iSplit]. by iApply adv_expr_low. by iApply adv_expr_low.
+      by iApply IH.
+    (* pairing *)
+    - move=>C1 IH e2 [] ??. rewrite low_ctx.
+      iSplit. by iApply IH. by iApply adv_expr_low.
+    - move=>e1 C2 IH [] ??. rewrite low_ctx.
+      iSplit. by iApply adv_expr_low. by iApply IH.
+    (* case *)
+    - move=>C0 IH e1 e2 [] ? [] ??. rewrite low_ctx.
+      iSplit; [|iSplit]. by iApply IH. by iApply adv_expr_low.
+      by iApply adv_expr_low.
+    - move=>e0 C1 IH e2 [] ? [] ??. rewrite low_ctx.
+      iSplit; [|iSplit]. by iApply adv_expr_low. by iApply IH.
+      by iApply adv_expr_low.
+    - move=>e0 e1 C2 IH [] ? [] ??. rewrite low_ctx.
+      iSplit; [|iSplit]. by iApply adv_expr_low. by iApply adv_expr_low.
+      by iApply IH.
+    (* store *)
+    - move=>C1 IH e2 [] ??. rewrite low_ctx.
+      iSplit. by iApply IH. by iApply adv_expr_low.
+    - move=>e1 C2 IH [] ??. rewrite low_ctx.
+      iSplit. by iApply adv_expr_low. by iApply IH.
+    (* CAS *)
+    - move=>C0 IH e1 e2 [] ? [] ??. rewrite low_ctx.
+      iSplit; [|iSplit]. by iApply IH. by iApply adv_expr_low.
+      by iApply adv_expr_low.
+    - move=>e0 C1 IH e2 [] ? [] ??. rewrite low_ctx.
+      iSplit; [|iSplit]. by iApply adv_expr_low. by iApply IH.
+      by iApply adv_expr_low.
+    - move=>e0 e1 C2 IH [] ? [] ??. rewrite low_ctx.
+      iSplit; [|iSplit]. by iApply adv_expr_low. by iApply adv_expr_low.
+      by iApply IH.
+  Qed.
+End adversary.
+
+(** * Robust safety *)
+(**
+	Our aim is to show that, under the heap invariant, if we plug
+	a closed, semantically low expression (i.e., verified code)
+	into a syntactically low context (i.e., an adversary), the
+	resulting expression is semantically low.
+
+	The proof is by induction on contexts, using the FTLR to zap
+	the context's subexpressions to low values. As in the proof of
+	the FTLR, we must generalize to account for substitution.
+ *)
+Section robust_safety.
+
+  Context `{heapG Σ}.
+  Implicit Types C : ctx.
+  Implicit Types e : expr.
+  Implicit Types v : val.
+  Existing Instance env_low.
+
+  Definition verified : pbit → expr → iProp Σ := λ p e, (
+     ⌜Closed [] e⌝ ∗ WP e @ p; ⊤ {{ low }}
+  )%I.
+
+  Definition safe : ctx → iProp Σ := λ C, (
+    ∀ Γ p e, heap_ctx -∗ low C -∗ low Γ -∗ □ verified p e -∗
+    WP substitute Γ (ctx_fill C e) ?{{ low }}
+  )%I.
+
+  Lemma verified_alt p e :
+    verified p e ⊣⊢
+    ⌜Closed [] e⌝ ∗ ∀ Φ, (∀ v, low v -∗ Φ v) -∗ WP e @ p; ⊤ {{ Φ }}.
+  Proof.
+    iSplit.
+    - iIntros "(%&He)". iSplit; first done. iIntros (Φ). by rewrite -wp_wand.
+    - iIntros "(%&He)". iSplit; first done. iApply "He". by iIntros.
+  Qed.
+
+  Lemma safe_alt C :
+    safe C ⊣⊢
+    ∀ Γ p e Φ, heap_ctx -∗ low C -∗ low Γ -∗ □ verified p e -∗
+    (∀ v, low v -∗ Φ v) -∗ WP substitute Γ (ctx_fill C e) ?{{ Φ }}.
+  Proof.
+    iSplit.
+    - iIntros "Hsafe". iIntros (Γ p e Φ) "Hh HC HΓ He".
+      rewrite -wp_wand. by iApply ("Hsafe" with "[$Hh] [$HC] [$HΓ] [$He]").
+    - iIntros "Halt". iIntros (Γ p e) "Hh HC HΓ He".
+      iApply ("Halt" with "[$Hh] [$HC] [$HΓ] [$He] []"). by iIntros.
+  Qed.
+
+  Lemma safe_hole : safe CHole.
+  Proof.
+    iIntros (Γ p e) "_ _ _ >(%&He) /=". iApply (wp_forget_progress p).
+    by rewrite substitute_closed.
+  Qed.
+
+  Lemma safe_rec f x C : □ safe C -∗ safe (CRec f x C).
+  Proof.
+    (* PDS: Lots of duplication with confined_rec. *)
+    iIntros "#IH". iIntros (Γ p e) "#Hh #HC #HΓ #He /=".
+    rewrite low_ctx substitute_expr. set erec := substitute _ _.
+    case: (decide (Closed (f :b: x :b: []) erec)) => ?;
+      last by iApply wp_stuck_rec_open.
+    iApply wp_value; first exact: to_val_rec.
+    rewrite/erec. set Γ' := (delete _ _).
+    iLöb as "Hvrec". rewrite {2}low_val. iAlways. iNext.
+    iIntros (v2) "#Hv2". case: (decide (x = f))=>?.
+    { subst. rewrite -> subst_subst'; last done.	(* ssr rewrite fails *)
+      rewrite of_val_rec subst_substitute; last by rewrite lookup_delete.
+      iApply ("IH" with "* [$Hh] [$HC] [] [He]"); last iExact "He". (* iNext bug *)
+      rewrite insert_delete. iApply (low_env_insert with "[$Hvrec] []");
+        first by rewrite lookup_delete.
+      by iApply (low_env_delete with "[$HΓ]"). }
+    rewrite of_val_rec subst_substitute; last by rewrite lookup_delete.
+    rewrite subst_substitute; last by rewrite
+      lookup_insert_ne // lookup_delete_ne // lookup_delete.
+    iApply ("IH" with "* [$Hh] [$HC] [] [He]"); last iExact "He". (* iNext bug *)
+    iApply (low_env_insert with "[$Hv2] []"); first by rewrite
+      lookup_insert_ne // lookup_delete_ne // lookup_delete.
+    iApply (low_env_insert with "[$Hvrec] []"); first by rewrite
+      lookup_delete.
+    do 2!iApply low_env_delete. iExact "HΓ".
+  Qed.
+
+  Lemma safe_app_l C1 e2 : safe C1 -∗ safe (CAppL C1 e2).
+  Proof.
+    rewrite (safe_alt (CAppL _ _)).
+    iIntros "IH". iIntros (Γ p e Φ) "#Hh Happ #HΓ He HΦ /=".
+    rewrite low_ctx substitute_expr. iDestruct "Happ" as "(HC1&He2)".
+    wp_bind (substitute _ _). rewrite safe_alt.
+    iApply ("IH" with "[$Hh] [$HC1] [$HΓ] [$He]"). iIntros (v1) "Hv1".
+    wp_bind (substitute _ _).
+    iApply (ftlr with "[$Hh] [$HΓ] [$He2]"); first done. iIntros (v2) "Hv2".
+    by iApply (wp_low_val_app with "[$Hv1 $Hv2] [$HΦ]").
+  Qed.
+
+  Lemma safe_app_r e1 C2 : safe C2 -∗ safe (CAppR e1 C2).
+  Proof.
+    rewrite (safe_alt (CAppR _ _)).
+    iIntros "IH". iIntros (Γ p e Φ) "#Hh Happ #HΓ He HΦ /=".
+    rewrite low_ctx substitute_expr. iDestruct "Happ" as "(He1&HC2)".
+    wp_bind (substitute _ _).
+    iApply (ftlr with "[$Hh] [$HΓ] [$He1]"); first done. iIntros (v1) "Hv1".
+    wp_bind (substitute _ _). rewrite safe_alt.
+    iApply ("IH" with "[$Hh] [$HC2] [$HΓ] [$He]"). iIntros (v2) "Hv2".
+    by iApply (wp_low_val_app with "[$Hv1 $Hv2] [$HΦ]").
+  Qed.
+
+  Lemma safe_un_op op C : safe C -∗ safe (CUnOp op C).
+  Proof.
+    rewrite (safe_alt (CUnOp _ _)).
+    iIntros "IH". iIntros (Γ p e Φ) "#Hh HC #HΓ He HΦ /=".
+    rewrite low_ctx substitute_expr.
+    wp_bind (substitute _ _). rewrite safe_alt.
+    iApply ("IH" with "[$Hh] [$HC] [$HΓ] [$He]"). iIntros (v) "_".
+    by iApply (wp_low_val_un_op with "[$HΦ]").
+  Qed.
+
+  Lemma safe_bin_op_l op C1 e2 : safe C1 -∗ safe (CBinOpL op C1 e2).
+  Proof.
+    rewrite (safe_alt (CBinOpL _ _ _)).
+    iIntros "IH". iIntros (Γ p e Φ) "#Hh Hop #HΓ He HΦ /=".
+    rewrite low_ctx substitute_expr. iDestruct "Hop" as "(HC1&He2)".
+    wp_bind (substitute _ _). rewrite safe_alt.
+    iApply ("IH" with "[$Hh] [$HC1] [$HΓ] [$He]"). iIntros (?) "_".
+    wp_bind (substitute _ _).
+    iApply (ftlr with "[$Hh] [$HΓ] [$He2]"); first done. iIntros (?) "_".
+    by iApply (wp_low_val_bin_op with "[$HΦ]").
+  Qed.
+
+  Lemma safe_bin_op_r op e1 C2 : safe C2 -∗ safe (CBinOpR op e1 C2).
+  Proof.
+    rewrite (safe_alt (CBinOpR _ _ _)).
+    iIntros "IH". iIntros (Γ p e Φ) "#Hh Hop #HΓ He HΦ /=".
+    rewrite low_ctx substitute_expr. iDestruct "Hop" as "(He1&HC2)".
+    wp_bind (substitute _ _).
+    iApply (ftlr with "[$Hh] [$HΓ] [$He1]"); first done. iIntros (?) "_".
+    wp_bind (substitute _ _). rewrite safe_alt.
+    iApply ("IH" with "[$Hh] [$HC2] [$HΓ] [$He]"). iIntros (?) "_".
+    by iApply (wp_low_val_bin_op with "[$HΦ]").
+  Qed.
+
+  Lemma safe_if C e1 e2 : safe C -∗ safe (CIf C e1 e2).
+  Proof.
+    rewrite (safe_alt (CIf _ _ _)).
+    iIntros "IH". iIntros (Γ p e Φ) "#Hh Hif #HΓ He HΦ /=".
+    rewrite low_ctx substitute_expr. iDestruct "Hif" as "(HC&He1&He2)".
+    wp_bind (substitute _ _). rewrite safe_alt.
+    iApply ("IH" with "[$Hh] [$HC] [$HΓ] [$He]"). iIntros (?) "_".
+    iApply wp_low_val_if. iNext. iSplit.
+    - by iApply (ftlr with "[$Hh] [$HΓ] [$He1] [$HΦ]").
+    - by iApply (ftlr with "[$Hh] [$HΓ] [$He2] [$HΦ]").
+  Qed.
+
+  Lemma safe_if_l e0 C1 e2 : safe C1 -∗ safe (CIfL e0 C1 e2).
+  Proof.
+    rewrite (safe_alt (CIfL _ _ _)).
+    iIntros "IH". iIntros (Γ p e Φ) "#Hh Hif #HΓ He HΦ /=".
+    rewrite low_ctx substitute_expr. iDestruct "Hif" as "(He0&HC1&He2)".
+    wp_bind (substitute _ _).
+    iApply (ftlr with "[$Hh] [$HΓ] [$He0]"); first done. iIntros (?) "_".
+    iApply wp_low_val_if. iNext. iSplit.
+    - rewrite safe_alt. by iApply ("IH" with "[$Hh] [$HC1] [$HΓ] [$He]").
+    - by iApply (ftlr with "[$Hh] [$HΓ] [$He2] [$HΦ]").
+  Qed.
+
+  Lemma safe_if_r e0 e1 C2 : safe C2 -∗ safe (CIfR e0 e1 C2).
+  Proof.
+    rewrite (safe_alt (CIfR _ _ _)).
+    iIntros "IH". iIntros (Γ p e Φ) "#Hh Hif #HΓ He HΦ /=".
+    rewrite low_ctx substitute_expr. iDestruct "Hif" as "(He0&He1&HC2)".
+    wp_bind (substitute _ _).
+    iApply (ftlr with "[$Hh] [$HΓ] [$He0]"); first done. iIntros (?) "_".
+    iApply wp_low_val_if. iNext. iSplit.
+    - by iApply (ftlr with "[$Hh] [$HΓ] [$He1] [$HΦ]").
+    - rewrite safe_alt. by iApply ("IH" with "[$Hh] [$HC2] [$HΓ] [$He]").
+  Qed.
+
+  Lemma safe_pair_l C1 e2 : safe C1 -∗ safe (CPairL C1 e2).
+  Proof.
+    rewrite (safe_alt (CPairL _ _)).
+    iIntros "IH". iIntros (Γ p e Φ) "#Hh Hp #HΓ He HΦ /=".
+    rewrite low_ctx substitute_expr. iDestruct "Hp" as "(HC1&He2)".
+    wp_bind (substitute _ _). rewrite safe_alt.
+    iApply ("IH" with "[$Hh] [$HC1] [$HΓ] [$He]"). iIntros (v1) "Hv1".
+    wp_bind (substitute _ _).
+    iApply (ftlr with "[$Hh] [$HΓ] [$He2]"); first done. iIntros (v2) "Hv2".
+    iApply wp_value; first by rewrite /= (to_of_val v1) (to_of_val v2).
+    iApply "HΦ". rewrite (low_val (PairV _ _)). by iFrame.
+  Qed.
+
+  Lemma safe_pair_r e1 C2 : safe C2 -∗ safe (CPairR e1 C2).
+  Proof.
+    rewrite (safe_alt (CPairR _ _)).
+    iIntros "IH". iIntros (Γ p e Φ) "#Hh Hp #HΓ He HΦ /=".
+    rewrite low_ctx substitute_expr. iDestruct "Hp" as "(He1&HC2)".
+    wp_bind (substitute _ _).
+    iApply (ftlr with "[$Hh] [$HΓ] [$He1]"); first done. iIntros (v1) "Hv1".
+    wp_bind (substitute _ _). rewrite safe_alt.
+    iApply ("IH" with "[$Hh] [$HC2] [$HΓ] [$He]"). iIntros (v2) "Hv2".
+    iApply wp_value; first by rewrite /= (to_of_val v1) (to_of_val v2).
+    iApply "HΦ". rewrite (low_val (PairV _ _)). by iFrame.
+  Qed.
+
+  Lemma safe_fst C : safe C -∗ safe (CFst C).
+  Proof.
+    rewrite (safe_alt (CFst _)).
+    iIntros "IH". iIntros (Γ p e Φ) "#Hh HC #HΓ He HΦ /=".
+    rewrite low_ctx substitute_expr.
+    wp_bind (substitute _ _). rewrite safe_alt.
+    iApply ("IH" with "[$Hh] [$HC] [$HΓ] [$He]"). iIntros (v) "Hv".
+    by iApply (wp_low_val_fst with "[$Hv] [$HΦ]").
+  Qed.
+
+  Lemma safe_snd C : safe C -∗ safe (CSnd C).
+  Proof.
+    rewrite (safe_alt (CSnd _)).
+    iIntros "IH". iIntros (Γ p e Φ) "#Hh HC #HΓ He HΦ /=".
+    rewrite low_ctx substitute_expr.
+    wp_bind (substitute _ _). rewrite safe_alt.
+    iApply ("IH" with "[$Hh] [$HC] [$HΓ] [$He]"). iIntros (v) "Hv".
+    by iApply (wp_low_val_snd with "[$Hv] [$HΦ]").
+  Qed.
+
+  Lemma safe_inl C : safe C -∗ safe (CInjL C).
+  Proof.
+    rewrite (safe_alt (CInjL _)).
+    iIntros "IH". iIntros (Γ p e Φ) "#Hh HC #HΓ He HΦ /=".
+    rewrite low_ctx substitute_expr.
+    wp_bind (substitute _ _). rewrite safe_alt.
+    iApply ("IH" with "[$Hh] [$HC] [$HΓ] [$He]"). iIntros (v) "Hv".
+    iApply wp_value; first by rewrite /= (to_of_val v).
+    iApply "HΦ". rewrite (low_val (InjLV _)). by iFrame.
+  Qed.
+
+  Lemma safe_inr C : safe C -∗ safe (CInjR C).
+  Proof.
+    rewrite (safe_alt (CInjR _)).
+    iIntros "IH". iIntros (Γ p e Φ) "#Hh HC #HΓ He HΦ /=".
+    rewrite low_ctx substitute_expr.
+    wp_bind (substitute _ _). rewrite safe_alt.
+    iApply ("IH" with "[$Hh] [$HC] [$HΓ] [$He]"). iIntros (v) "Hv".
+    iApply wp_value; first by rewrite /= (to_of_val v).
+    iApply "HΦ". rewrite (low_val (InjRV _)). by iFrame.
+  Qed.
+
+  Lemma safe_case C e1 e2 : safe C -∗ safe (CCase C e1 e2).
+  Proof.
+    rewrite (safe_alt (CCase _ _ _)).
+    iIntros "IH". iIntros (Γ p e Φ) "#Hh Hc #HΓ He HΦ /=".
+    rewrite low_ctx substitute_expr. iDestruct "Hc" as "(HC&He1&He2)".
+    wp_bind (substitute _ _). rewrite safe_alt.
+    iApply ("IH" with "[$Hh] [$HC] [$HΓ] [$He]"). iIntros (v) "Hv".
+    iApply (wp_low_val_case with "[$Hv]"). iNext. iIntros (v0) "#Hv0".
+    iSplit; wp_bind (substitute _ _).
+    - iApply (ftlr with "[$Hh] [$HΓ] [$He1]"); first done. iIntros (v1) "Hv1".
+      by iApply (wp_low_val_app with "[$Hv1 $Hv0] [$HΦ]").
+    - iApply (ftlr with "[$Hh] [$HΓ] [$He2]"); first done. iIntros (v2) "Hv2".
+      by iApply (wp_low_val_app with "[$Hv2 $Hv0] [$HΦ]").
+  Qed.
+
+  Lemma safe_case_l e0 C1 e2 : safe C1 -∗ safe (CCaseL e0 C1 e2).
+  Proof.
+    rewrite (safe_alt (CCaseL _ _ _)).
+    iIntros "IH". iIntros (Γ p e Φ) "#Hh Hc #HΓ He HΦ /=".
+    rewrite low_ctx substitute_expr. iDestruct "Hc" as "(He0&HC1&He2)".
+    wp_bind (substitute _ _).
+    iApply (ftlr with "[$Hh] [$HΓ] [$He0]"); first done. iIntros (v) "Hv".
+    iApply (wp_low_val_case with "[$Hv]"). iNext. iIntros (v0) "#Hv0".
+    iSplit; wp_bind (substitute _ _).
+    - rewrite safe_alt.
+      iApply ("IH" with "[$Hh] [$HC1] [$HΓ] [$He]"). iIntros (v1) "Hv1".
+      by iApply (wp_low_val_app with "[$Hv1 $Hv0] [$HΦ]").
+    - iApply (ftlr with "[$Hh] [$HΓ] [$He2]"); first done. iIntros (v2) "Hv2".
+      by iApply (wp_low_val_app with "[$Hv2 $Hv0] [$HΦ]").
+  Qed.
+
+  Lemma safe_case_r e0 e1 C2 : safe C2 -∗ safe (CCaseR e0 e1 C2).
+  Proof.
+    rewrite (safe_alt (CCaseR _ _ _)).
+    iIntros "IH". iIntros (Γ p e Φ) "#Hh Hc #HΓ He HΦ /=".
+    rewrite low_ctx substitute_expr. iDestruct "Hc" as "(He0&He1&HC2)".
+    wp_bind (substitute _ _).
+    iApply (ftlr with "[$Hh] [$HΓ] [$He0]"); first done. iIntros (v) "Hv".
+    iApply (wp_low_val_case with "[$Hv]"). iNext. iIntros (v0) "#Hv0".
+    iSplit; wp_bind (substitute _ _).
+    - iApply (ftlr with "[$Hh] [$HΓ] [$He1]"); first done. iIntros (v1) "Hv1".
+      by iApply (wp_low_val_app with "[$Hv1 $Hv0] [$HΦ]").
+    - rewrite safe_alt.
+      iApply ("IH" with "[$Hh] [$HC2] [$HΓ] [$He]"). iIntros (v2) "Hv2".
+      by iApply (wp_low_val_app with "[$Hv2 $Hv0] [$HΦ]").
+  Qed.
+
+  Lemma safe_assert C : safe (CAssert C).
+  Proof. iIntros (Γ p e) "_ Hc _ _ /=". rewrite low_ctx. by iExFalso. Qed.
+
+  Lemma safe_fork C : safe C -∗ safe (CFork C).
+  Proof.
+    rewrite (safe_alt (CFork _)).
+    iIntros "IH". iIntros (Γ p e Φ) "#Hh HC #HΓ He HΦ /=".
+    rewrite low_ctx substitute_expr. iApply wp_fork. iNext. iSplitL "HΦ".
+    - iApply "HΦ". by rewrite low_val low_lit.
+    - rewrite safe_alt. iApply ("IH" with "[$Hh] [$HC] [$HΓ] [$He]").
+      by iIntros.
+  Qed.
+
+  Lemma safe_alloc C : safe C -∗ safe (CAlloc C).
+  Proof.
+    rewrite (safe_alt (CAlloc _)).
+    iIntros "IH". iIntros (Γ p e Φ) "#Hh HC #HΓ He HΦ /=".
+    rewrite low_ctx substitute_expr.
+    wp_bind (substitute _ _). rewrite safe_alt.
+    iApply ("IH" with "[$Hh] [$HC] [$HΓ] [$He]"). iIntros (v) "Hv".
+    iApply (wp_alloc_low with "[$Hh $Hv]"); [by rewrite to_of_val|done|].
+    iNext. iIntros (l) "#Hl". iApply "HΦ". by rewrite low_val low_lit.
+  Qed.
+
+  Lemma safe_load C : safe C -∗ safe (CLoad C).
+  Proof.
+    rewrite (safe_alt (CLoad _)).
+    iIntros "IH". iIntros (Γ p e Φ) "#Hh HC #HΓ He HΦ /=".
+    rewrite low_ctx substitute_expr.
+    wp_bind (substitute _ _). rewrite safe_alt.
+    iApply ("IH" with "[$Hh] [$HC] [$HΓ] [$He]"). iIntros (v) "Hv".
+    by iApply (wp_low_val_load with "[$Hh $Hv] [$HΦ]").
+  Qed.
+
+  Lemma safe_store_l C1 e2 : safe C1 -∗ safe (CStoreL C1 e2).
+  Proof.
+    rewrite (safe_alt (CStoreL _ _)).
+    iIntros "IH". iIntros (Γ p e Φ) "#Hh Hp #HΓ He HΦ /=".
+    rewrite low_ctx substitute_expr. iDestruct "Hp" as "(HC1&He2)".
+    wp_bind (substitute _ _). rewrite safe_alt.
+    iApply ("IH" with "[$Hh] [$HC1] [$HΓ] [$He]"). iIntros (v1) "Hv1".
+    wp_bind (substitute _ _).
+    iApply (ftlr with "[$Hh] [$HΓ] [$He2]"); first done. iIntros (v2) "Hv2".
+    by iApply (wp_low_val_store with "[$Hh $Hv1 $Hv2] [$HΦ]").
+  Qed.
+
+  Lemma safe_store_r e1 C2 : safe C2 -∗ safe (CStoreR e1 C2).
+  Proof.
+    rewrite (safe_alt (CStoreR _ _)).
+    iIntros "IH". iIntros (Γ p e Φ) "#Hh Hp #HΓ He HΦ /=".
+    rewrite low_ctx substitute_expr. iDestruct "Hp" as "(He1&HC2)".
+    wp_bind (substitute _ _).
+    iApply (ftlr with "[$Hh] [$HΓ] [$He1]"); first done. iIntros (v1) "Hv1".
+    wp_bind (substitute _ _). rewrite safe_alt.
+    iApply ("IH" with "[$Hh] [$HC2] [$HΓ] [$He]"). iIntros (v2) "Hv2".
+    by iApply (wp_low_val_store with "[$Hh $Hv1 $Hv2] [$HΦ]").
+  Qed.
+
+  Lemma safe_cas_l C e1 e2 : safe C -∗ safe (CCASL C e1 e2).
+  Proof.
+    rewrite (safe_alt (CCASL _ _ _)).
+    iIntros "IH". iIntros (Γ p e Φ) "#Hh Hc #HΓ He HΦ /=".
+    rewrite low_ctx substitute_expr. iDestruct "Hc" as "(HC&He1&He2)".
+    wp_bind (substitute _ _). rewrite safe_alt.
+    iApply ("IH" with "[$Hh] [$HC] [$HΓ] [$He]"). iIntros (v0) "Hv0".
+    wp_bind (substitute _ _).
+    iApply (ftlr with "[$Hh] [$HΓ] [$He1]"); first done. iIntros (v1) "_".
+    wp_bind (substitute _ _).
+    iApply (ftlr with "[$Hh] [$HΓ] [$He2]"); first done. iIntros (v2) "Hv2".
+    by iApply (wp_low_val_cas with "[$Hh $Hv0 $Hv2] [$HΦ]").
+  Qed.
+
+  Lemma safe_cas_m e0 C1 e2 : safe C1 -∗ safe (CCASM e0 C1 e2).
+  Proof.
+    rewrite (safe_alt (CCASM _ _ _)).
+    iIntros "IH". iIntros (Γ p e Φ) "#Hh Hc #HΓ He HΦ /=".
+    rewrite low_ctx substitute_expr. iDestruct "Hc" as "(He0&HC1&He2)".
+    wp_bind (substitute _ _).
+    iApply (ftlr with "[$Hh] [$HΓ] [$He0]"); first done. iIntros (v0) "Hv0".
+    wp_bind (substitute _ _). rewrite safe_alt.
+    iApply ("IH" with "[$Hh] [$HC1] [$HΓ] [$He]"). iIntros (v1) "Hv1".
+    wp_bind (substitute _ _).
+    iApply (ftlr with "[$Hh] [$HΓ] [$He2]"); first done. iIntros (v2) "Hv2".
+    by iApply (wp_low_val_cas with "[$Hh $Hv0 $Hv2] [$HΦ]").
+  Qed.
+
+  Lemma safe_cas_r e0 e1 C2 : safe C2 -∗ safe (CCASR e0 e1 C2).
+  Proof.
+    rewrite (safe_alt (CCASR _ _ _)).
+    iIntros "IH". iIntros (Γ p e Φ) "#Hh Hc #HΓ He HΦ /=".
+    rewrite low_ctx substitute_expr. iDestruct "Hc" as "(He0&He1&HC2)".
+    wp_bind (substitute _ _).
+    iApply (ftlr with "[$Hh] [$HΓ] [$He0]"); first done. iIntros (v0) "Hv0".
+    wp_bind (substitute _ _).
+    iApply (ftlr with "[$Hh] [$HΓ] [$He1]"); first done. iIntros (v1) "_".
+    wp_bind (substitute _ _). rewrite safe_alt.
+    iApply ("IH" with "[$Hh] [$HC2] [$HΓ] [$He]"). iIntros (v2) "Hv2".
+    by iApply (wp_low_val_cas with "[$Hh $Hv0 $Hv2] [$HΦ]").
+  Qed.
+
+  Theorem robust_safety' C : safe C.
+  Proof.
+    iStartProof.
+    iInduction C as [| | | | | | | | | | | | | | | | | | | | | | | | | | |] "IH".
+    - by rewrite -safe_hole.
+    - by rewrite -safe_rec.
+    - by rewrite -safe_app_l.
+    - by rewrite -safe_app_r.
+    - by rewrite -safe_un_op.
+    - by rewrite -safe_bin_op_l.
+    - by rewrite -safe_bin_op_r.
+    - by rewrite -safe_if.
+    - by rewrite -safe_if_l.
+    - by rewrite -safe_if_r.
+    - by rewrite -safe_pair_l.
+    - by rewrite -safe_pair_r.
+    - by rewrite -safe_fst.
+    - by rewrite -safe_snd.
+    - by rewrite -safe_inl.
+    - by rewrite -safe_inr.
+    - by rewrite -safe_case.
+    - by rewrite -safe_case_l.
+    - by rewrite -safe_case_r.
+    - by rewrite -safe_assert.
+    - by rewrite -safe_fork.
+    - by rewrite -safe_alloc.
+    - by rewrite -safe_load.
+    - by rewrite -safe_store_l.
+    - by rewrite -safe_store_r.
+    - by rewrite -safe_cas_l.
+    - by rewrite -safe_cas_m.
+    - by rewrite -safe_cas_r.
+  Qed.
+End robust_safety.
