theories/tests/barrier_client.v
@@ -13,9 +13,7 @@ Definition client : expr :=
     (worker 12 "b" "y" ||| worker 17 "b" "y").
 
 Section client.
-  Context `{!heapG Σ, !barrierG Σ, !spawnG Σ}.
-
-  Local Definition N := nroot .@ "barrier".
+  Context `{!heapG Σ, !barrierG Σ, !spawnG Σ} (N : namespace).
 
   Definition y_inv (q : Qp) (l : loc) : iProp Σ :=
     (∃ f : val, l ↦{q} f ∗ □ ∀ n : Z, WP f #n {{ v, ⌜v = #(n + 42)⌝ }})%I.
@@ -27,20 +25,20 @@ Section client.
   Qed.
 
   Lemma worker_safe q (n : Z) (b y : loc) :
-    recv N b (y_inv q y) -∗ WP worker n #b #y {{ _, True }}.
+    heap_ctx -∗ recv N b (y_inv q y) -∗ WP worker n #b #y {{ _, True }}.
   Proof.
-    iIntros "Hrecv". wp_lam. wp_let.
-    wp_apply (wait_spec with "Hrecv"). iDestruct 1 as (f) "[Hy #Hf]".
+    iIntros "#Hh Hrecv". wp_lam. wp_let.
+    wp_apply (wait_spec with "[- $Hrecv]"). iDestruct 1 as (f) "[Hy #Hf]".
     wp_seq. wp_load.
     iApply (wp_wand with "[]"). iApply "Hf". by iIntros (v) "_".
   Qed.
 
-  Lemma client_safe : WP client {{ _, True }}%I.
+  Lemma client_safe : heapN ⊥ N → heap_ctx -∗ WP client {{ _, True }}%I.
   Proof.
-    iIntros ""; rewrite /client. wp_alloc y as "Hy". wp_let.
-    wp_apply (newbarrier_spec N (y_inv 1 y)).
+    iIntros (?) "#Hh"; rewrite /client. wp_alloc y as "Hy". wp_let.
+    wp_apply (newbarrier_spec N (y_inv 1 y) with "Hh"); first done.
     iIntros (l) "[Hr Hs]". wp_let.
-    iApply (wp_par (λ _, True%I) (λ _, True%I) with "[Hy Hs] [Hr]"); last auto.
+    iApply (wp_par (λ _, True%I) (λ _, True%I) with "[$Hh] [Hy Hs] [Hr]"); last auto.
     - (* The original thread, the sender. *)
       wp_store. iApply (signal_spec with "[-]"); last by iNext; auto.
       iSplitR "Hy"; first by eauto.
@@ -49,9 +47,9 @@ Section client.
       iDestruct (recv_weaken with "[] Hr") as "Hr".
       { iIntros "Hy". by iApply (y_inv_split with "Hy"). }
       iMod (recv_split with "Hr") as "[H1 H2]"; first done.
-      iApply (wp_par (λ _, True%I) (λ _, True%I) with "[H1] [H2]"); last auto.
-      + by iApply worker_safe.
-      + by iApply worker_safe.
+      iApply (wp_par (λ _, True%I) (λ _, True%I) with "[$Hh] [H1] [H2]"); last auto.
+      + by iApply (worker_safe with "Hh").
+      + by iApply (worker_safe with "Hh").
 Qed.
 End client.
 
@@ -59,8 +57,12 @@ Section ClosedProofs.
 
 Let Σ : gFunctors := #[ heapΣ ; barrierΣ ; spawnΣ ].
 
-Lemma client_adequate σ : adequate progress client σ (λ _, True).
-Proof. apply (heap_adequacy Σ)=> ?. apply client_safe. Qed.
+Lemma client_adequate h :
+  adequate progress client (good_state h) (λ _, True).
+Proof.
+  apply (heap_adequacy Σ)=> ?.
+  apply (client_safe (nroot .@ "barrier")); auto with ndisj.
+Qed.
 
 End ClosedProofs.
 
